Interface for Pointer

ulib/FStar.Pointer.fst
@@ -8,109 +8,6 @@ open HST // for := , !
 
 (*** Definitions *)
 
-(** Type codes *)
-
-type base_typ =
-| TUInt
-| TUInt8
-| TUInt16
-| TUInt32
-| TUInt64
-| TInt
-| TInt8
-| TInt16
-| TInt32
-| TInt64
-| TChar
-| TBool
-| TUnit
-
-// C11, Sect. 6.2.5 al. 20: arrays must be nonempty
-type array_length_t = (length: UInt32.t { UInt32.v length > 0 } )
-
-type typ =
-| TBase:
-  (b: base_typ) ->
-  typ
-| TStruct:
-  (l: struct_typ) ->
-  typ
-| TUnion:
-  (l: union_typ) ->
-  typ
-| TArray:
-  (length: array_length_t ) ->
-  (t: typ) ->
-  typ
-| TPointer:
-  (t: typ) ->
-  typ
-| TNPointer:
-  (t: typ) ->
-  typ
-| TBuffer:
-  (t: typ) ->
-  typ
-and struct_typ = (l: list (string * typ) {
-  Cons? l /\ // C11, 6.2.5 al. 20: structs and unions must have at least one field
-  List.Tot.noRepeats (List.Tot.map fst l)
-})
-and union_typ = struct_typ
-
-(** `struct_field l` is the type of fields of `TStruct l`
-    (i.e. a refinement of `string`).
-*)
-let struct_field
-  (l: struct_typ)
-: Tot eqtype
-= (s: string { List.Tot.mem s (List.Tot.map fst l) } )
-
-(** `typ_of_struct_field l f` is the type of data associated with field `f` in
-    `TStruct l` (i.e. a refinement of `typ`).
-*)
-let typ_of_struct_field
-  (l: struct_typ)
-  (f: struct_field l)
-: Tot (t: typ {t << l})
-= List.Tot.assoc_mem f l;
-  let y = Some?.v (List.Tot.assoc f l) in
-  List.Tot.assoc_precedes f l y;
-  y
-
-let rec typ_depth
-  (t: typ)
-: GTot nat
-= match t with
-  | TArray _ t -> 1 + typ_depth t
-  | TUnion l
-  | TStruct l -> 1 + struct_typ_depth l
-  | _ -> 0
-and struct_typ_depth
-  (l: list (string * typ))
-: GTot nat
-= match l with
-  | [] -> 0
-  | (_, t) :: l ->
-    let n1 = typ_depth t in
-    let n2 = struct_typ_depth l in
-    if n1 > n2 then n1 else n2
-
-let rec typ_depth_typ_of_struct_field
-  (l: struct_typ)
-  (f: struct_field l)
-: Lemma
-  (ensures (typ_depth (typ_of_struct_field l f) <= struct_typ_depth l))
-  (decreases l)
-= let ((f', _) :: l') = l in
-  if f = f'
-  then ()
-  else begin
-    let f: string = f in
-    assert (List.Tot.mem f (List.Tot.map fst l'));
-    List.Tot.assoc_mem f l';
-    typ_depth_typ_of_struct_field l' f
-  end
-
 (** Pointers to data of type t.
 
     This defines two main types:
@@ -121,7 +18,7 @@ let rec typ_depth_typ_of_struct_field
     `nullptr #t` (of type `npointer t`) represents the "NULL" value.
 *)
 
-private type step: (from: typ) -> (to: typ) -> Tot Type0 =
+type step: (from: typ) -> (to: typ) -> Tot Type0 =
   | StepField:
     (l: struct_typ) ->
     (fd: struct_field l) ->
@@ -136,7 +33,7 @@ private type step: (from: typ) -> (to: typ) -> Tot Type0 =
     (index: UInt32.t { UInt32.v index < UInt32.v length } ) ->
     step (TArray length value) value
 
-private type path (from: typ) : (to: typ) -> Tot Type0 =
+type path (from: typ) : (to: typ) -> Tot Type0 =
   | PathBase:
     path from from
   | PathStep:
@@ -146,7 +43,7 @@ private type path (from: typ) : (to: typ) -> Tot Type0 =
     (s: step through to) ->
     path from to
 
-private let step_typ_depth
+let step_typ_depth
   (#from #to: typ)
   (s: step from to)
 : Lemma
@@ -157,7 +54,7 @@ private let step_typ_depth
     typ_depth_typ_of_struct_field l fd
   | _ -> ()
 
-private let rec path_typ_depth
+let rec path_typ_depth
   (#from #to: typ)
   (p: path from to)
 : Lemma
@@ -199,7 +96,7 @@ private let path' (from: typ) (to: typ) : Tot Type0 =
   else path from to
 *)
 
-noeq private type _npointer (to : typ): Type0 =
+noeq type _npointer (to : typ): Type0 =
   | Pointer:
     (from: typ) ->
     (contents: HS.aref) ->
@@ -207,31 +104,28 @@ noeq private type _npointer (to : typ): Type0 =
     _npointer to
   | NullPtr
 
-abstract let npointer (t: typ): Tot Type0 =
+let npointer (t: typ): Tot Type0 =
   _npointer t
 
 (** The null pointer *)
 
-abstract let nullptr (#t: typ): Tot (npointer t) = NullPtr
+let nullptr (#t: typ): Tot (npointer t) = NullPtr
 
-abstract let g_is_null (#t: typ) (p: npointer t) : GTot bool =
+let g_is_null (#t: typ) (p: npointer t) : GTot bool =
   match p with
   | NullPtr -> true
   | _ -> false
 
-abstract let g_is_null_intro
+let g_is_null_intro
   (t: typ)
 : Lemma
   (g_is_null (nullptr #t) == true)
   [SMTPat (g_is_null (nullptr #t))]
 = ()
 
-// concrete, for subtyping
-let pointer (t: typ) : Tot Type0 = (p: npointer t { g_is_null p == false } )
-
 (** Buffers *)
 
-noeq private type buffer_root (t: typ) =
+noeq type buffer_root (t: typ) =
 | BufferRootSingleton:
   (p: pointer t) ->
   buffer_root t
@@ -240,58 +134,17 @@ noeq private type buffer_root (t: typ) =
   (p: pointer (TArray max_length t)) ->
   buffer_root t
 
-private let buffer_root_length (#t: typ) (b: buffer_root t): Tot UInt32.t = match b with
+let buffer_root_length (#t: typ) (b: buffer_root t): Tot UInt32.t = match b with
 | BufferRootSingleton _ -> 1ul
 | BufferRootArray #t #len _ -> len
 
-noeq private type _buffer (t: typ) =
+noeq type _buffer (t: typ) =
 | Buffer:
   (broot: buffer_root t) ->
   (bidx: UInt32.t) ->
   (blength: UInt32.t { UInt32.v bidx + UInt32.v blength <= UInt32.v (buffer_root_length broot) } ) ->
   _buffer t
-abstract let buffer (t: typ): Tot Type0 = _buffer t
-
-(** Interpretation of type codes.
-
-   Defines functions mapping from type codes (`typ`) to their interpretation as
-   FStar types. For example, `type_of_typ (TBase TUInt8)` is `FStar.UInt8.t`.
-*)
-
-(** Interpretation of base types. *)
-let type_of_base_typ
-  (t: base_typ)
-: Tot Type0
-= match t with
-  | TUInt -> nat
-  | TUInt8 -> FStar.UInt8.t
-  | TUInt16 -> FStar.UInt16.t
-  | TUInt32 -> FStar.UInt32.t
-  | TUInt64 -> FStar.UInt64.t
-  | TInt -> int
-  | TInt8 -> FStar.Int8.t
-  | TInt16 -> FStar.Int16.t
-  | TInt32 -> FStar.Int32.t
-  | TInt64 -> FStar.Int64.t
-  | TChar -> FStar.Char.char
-  | TBool -> bool
-  | TUnit -> unit
-
-(** Interpretation of arrays of elements of (interpreted) type `t`. *)
-type array (length: array_length_t) (t: Type) = (s: Seq.seq t {Seq.length s == UInt32.v length})
-
-let type_of_struct_field'
-  (l: struct_typ)
-  (type_of_typ: (
-    (t: typ { t << l } ) ->
-    Tot Type0
-  ))
-  (f: struct_field l)
-: Tot Type0 =
-  List.Tot.assoc_mem f l;
-  let y = typ_of_struct_field l f in
-  List.Tot.assoc_precedes f l y;
-  type_of_typ y
+let buffer (t: typ): Tot Type0 = _buffer t
 
 (** Helper for the interpretation of unions.
 
@@ -304,14 +157,13 @@ let type_of_struct_field'
     - `gtdata_get_value` asks for the key `k` to read, and a proof that `k`
       matches the ghost key.
 *)
-abstract
+
 let gtdata (* ghostly-tagged data *)
-  (key: eqtype)
+  (key: eqtype u#0)
   (value: (key -> Tot Type0))
 : Tot Type0
 = ( k: key & value k )
 
-private
 let _gtdata_get_key
   (#key: eqtype)
   (#value: (key -> Tot Type0))
@@ -319,12 +171,6 @@ let _gtdata_get_key
 : Tot key
 = dfst u
 
-(** Gets the current tag (or key) of a union.
-
-    This is a ghost function, as this tag only exists at the logical level and
-    is not stored in memory.
-*)
-abstract
 let gtdata_get_key
   (#key: eqtype)
   (#value: (key -> Tot Type0))
@@ -332,12 +178,6 @@ let gtdata_get_key
 : GTot key // important: must be Ghost, the tag is not actually stored in memory
 = _gtdata_get_key u
 
-(** Gets the value of a union, provided the field to read from.
-
-    This field must match the ghost tag of the union (hence the `require`
-    clause).
-*)
-abstract
 let gtdata_get_value
   (#key: eqtype)
   (#value: (key -> Tot Type0))
@@ -348,7 +188,6 @@ let gtdata_get_value
   (ensures (fun _ -> True))
 = let (| _, v |) = u in v
 
-abstract
 let gtdata_create
   (#key: eqtype)
   (#value: (key -> Tot Type0))
@@ -359,7 +198,6 @@ let gtdata_create
   (ensures (fun x -> gtdata_get_key x == k /\ gtdata_get_value x k == v))
 = (| k, v |)
 
-abstract
 let gtdata_extensionality
   (#key: eqtype)
   (#value: (key -> Tot Type0))
@@ -373,170 +211,15 @@ let gtdata_extensionality
   (ensures (u1 == u2))
 = ()
 
-(* Interperets a type code (`typ`) as a FStar type (`Type0`). *)
-let rec type_of_typ
-  (t: typ)
-: Tot Type0
-= match t with
-  | TBase b -> type_of_base_typ b
-  | TStruct l ->
-    DM.t (struct_field l) (type_of_struct_field' l type_of_typ)
-  | TUnion l ->
-    gtdata (struct_field l) (type_of_struct_field' l type_of_typ)
-  | TArray length t ->
-    array length (type_of_typ t)
-  | TPointer t ->
-    pointer t
-  | TNPointer t ->
-    npointer t
-  | TBuffer t ->
-    buffer t
-
-let type_of_struct_field
-  (l: struct_typ)
-: Tot (struct_field l -> Tot Type0)
-= type_of_struct_field' l type_of_typ
-
-(** Interpretation of structs, as dependent maps. *)
-let struct (l: struct_typ) = DM.t (struct_field l) (type_of_struct_field l)
-
-let type_of_typ_struct
-  (l: struct_typ)
-: Lemma
-  (type_of_typ (TStruct l) == struct l)
-  [SMTPat (type_of_typ (TStruct l))]
-= assert_norm (type_of_typ (TStruct l) == struct l)
-
-let type_of_typ_type_of_struct_field
-  (l: struct_typ)
-  (f: struct_field l)
-: Lemma
-  (type_of_typ (typ_of_struct_field l f) == type_of_struct_field l f)
-  [SMTPat (type_of_typ (typ_of_struct_field l f))]
-= ()
-
-let struct_sel (#l: struct_typ) (s: struct l) (f: struct_field l) : Tot (type_of_struct_field l f) =
-  DM.sel s f
-
-let struct_upd (#l: struct_typ) (s: struct l) (f: struct_field l) (v: type_of_struct_field l f) : Tot (struct l) =
-  DM.upd s f v
-
-let dfst_struct_field
-  (s: struct_typ)
-  (p: (x: struct_field s & type_of_struct_field s x))
-: Tot string
-=
-  let (| f, _ |) = p in
-  f
-
-(* TODO move to FStar.List.Tot.Properties *)
-
-let rec find_none
-  (#a: Type)
-  (f: (a -> Tot bool))
-  (l: list a)
-  (x: a)
-: Lemma
-  (requires (List.Tot.find f l == None /\ List.Tot.memP x l))
-  (ensures (f x == false))
-= let (x' :: l') = l in
-  Classical.or_elim
-    #(x == x')
-    #(~ (x == x'))
-    #(fun _ -> f x == false)
-    (fun h -> ())
-    (fun h -> find_none f l' x)
-
-let rec mem_count
-  (#a: eqtype)
-  (l: list a)
-  (x: a)
-: Lemma
-  (List.Tot.mem x l <==> List.Tot.count x l > 0)
-= match l with
-  | [] -> ()
-  | x' :: l' -> mem_count l' x
-
-let struct_literal (s: struct_typ) : Tot Type0 = (list (x: struct_field s & type_of_struct_field s x))
-
-let struct_literal_wf (s: struct_typ) (l: struct_literal s) : Tot bool =
-  List.Tot.sortWith FStar.String.compare (List.Tot.map fst s) =
-  List.Tot.sortWith FStar.String.compare
-    (List.Tot.map (dfst_struct_field s) l)
-
-let fun_of_list
-  (s: struct_typ)
-  (l: struct_literal s)
-  (f: struct_field s)
-: Pure (type_of_struct_field s f)
-  (requires (normalize_term (struct_literal_wf s l) == true))
-  (ensures (fun _ -> True))
-=
-  let f' : string = f in
-  let phi (p: (x: struct_field s & type_of_struct_field s x)) : Tot bool =
-    dfst_struct_field s p = f'
-  in
-  match List.Tot.find phi l with
-  | Some p -> let (| _, v |) = p in v
-  | _ ->
-    List.Tot.sortWith_permutation FStar.String.compare (List.Tot.map fst s);
-    List.Tot.sortWith_permutation FStar.String.compare (List.Tot.map (dfst_struct_field s) l);
-    List.Tot.mem_memP f' (List.Tot.map fst s);
-    mem_count (List.Tot.map fst s) f';
-    mem_count (List.Tot.map (dfst_struct_field s) l) f';
-    List.Tot.mem_memP f' (List.Tot.map (dfst_struct_field s) l);
-    List.Tot.memP_map_elim (dfst_struct_field s) f' l;
-    Classical.forall_intro (Classical.move_requires (find_none phi l));
-    false_elim ()
-
-let struct_create (l: struct_typ) (f: ((fd: struct_field l) -> Tot (type_of_struct_field l fd))) : Tot (struct l) =
-  DM.create #(struct_field l) #(type_of_struct_field l) f
-
-let struct_create'
-  (s: struct_typ)
-  (l: struct_literal s)
-: Pure (struct s)
-  (requires (normalize_term (struct_literal_wf s l) == true))
-  (ensures (fun _ -> True))
-= struct_create s (fun_of_list s l)
-
 (** Interpretation of unions, as ghostly-tagged data
     (see `gtdata` for more information).
 *)
-let union (l: struct_typ) = gtdata (struct_field l) (type_of_struct_field l)
-
-let type_of_typ_union
-  (l: union_typ)
-: Lemma
-  (type_of_typ (TUnion l) == union l)
-  [SMTPat (type_of_typ (TUnion l))]
-= assert_norm (type_of_typ (TUnion l) == union l)
-
-private let _union_get_key (#l: union_typ) (v: union l) : Tot (struct_field l) = _gtdata_get_key v
-
-let union_get_key (#l: union_typ) (v: union l) : GTot (struct_field l) = gtdata_get_key v
-
-let union_get_value
-  (#l: union_typ)
-  (v: union l)
-  (fd: struct_field l)
-: Pure (type_of_struct_field l fd)
-  (requires (union_get_key v == fd))
-  (ensures (fun _ -> True))
-= gtdata_get_value v fd
-
-let union_create
-  (l: union_typ)
-  (fd: struct_field l)
-  (v: type_of_struct_field l fd)
-: Tot (union l)
-= gtdata_create fd v
+let _union_get_key (#l: union_typ) (v: union l) : Tot (struct_field l) = _gtdata_get_key v
 
 (** For any `t: typ`, `dummy_val t` provides a default value of this type.
 
     This is useful to represent uninitialized data.
 *)
-private
 let rec dummy_val
   (t: typ)
 : Tot (type_of_typ t)
@@ -595,7 +278,6 @@ let rec dummy_val
       therefore that reading uninitialized data is actually forbidden.
 *)
 
-private
 let rec otype_of_typ
   (t: typ)
 : Tot Type0
@@ -614,13 +296,11 @@ let rec otype_of_typ
   | TBuffer t ->
     option (buffer t)
 
-private
 let otype_of_struct_field
   (l: struct_typ)
 : Tot (struct_field l -> Tot Type0)
 = type_of_struct_field' l otype_of_typ
 
-private
 let otype_of_typ_otype_of_struct_field
   (l: struct_typ)
   (f: struct_field l)
@@ -629,7 +309,6 @@ let otype_of_typ_otype_of_struct_field
   [SMTPat (type_of_typ (typ_of_struct_field l f))]
 = ()
 
-private
 let otype_of_typ_base
   (b: base_typ)
 : Lemma
@@ -637,7 +316,6 @@ let otype_of_typ_base
   [SMTPat (otype_of_typ (TBase b))]
 = ()
 
-private
 let otype_of_typ_array
   (len: array_length_t )
   (t: typ)
@@ -646,22 +324,17 @@ let otype_of_typ_array
   [SMTPat (otype_of_typ (TArray len t))]
 = ()
 
-private
 let ostruct (l: struct_typ) = option (DM.t (struct_field l) (otype_of_struct_field l))
 
-private
 let ostruct_sel (#l: struct_typ) (s: ostruct l { Some? s }) (f: struct_field l) : Tot (otype_of_struct_field l f) =
   DM.sel (Some?.v s) f
 
-private
 let ostruct_upd (#l: struct_typ) (s: ostruct l { Some? s }) (f: struct_field l) (v: otype_of_struct_field l f) : Tot (s': ostruct l { Some? s' } ) =
   Some (DM.upd (Some?.v s) f v)
 
-private
 let ostruct_create (l: struct_typ) (f: ((fd: struct_field l) -> Tot (otype_of_struct_field l fd))) : Tot (s': ostruct l { Some? s' } ) =
   Some (DM.create #(struct_field l) #(otype_of_struct_field l) f)
 
-private
 let otype_of_typ_struct
   (l: struct_typ)
 : Lemma
@@ -669,12 +342,10 @@ let otype_of_typ_struct
   [SMTPat (otype_of_typ (TStruct l))]
 = assert_norm(otype_of_typ (TStruct l) == ostruct l)
 
-private
 let ounion (l: struct_typ) = option (gtdata (struct_field l) (otype_of_struct_field l))
 
-private let ounion_get_key (#l: union_typ) (v: ounion l { Some? v } ) : Tot (struct_field l) = _gtdata_get_key (Some?.v v)
+let ounion_get_key (#l: union_typ) (v: ounion l { Some? v } ) : Tot (struct_field l) = _gtdata_get_key (Some?.v v)
 
-private
 let ounion_get_value
   (#l: union_typ)
   (v: ounion l { Some? v } )
@@ -684,7 +355,6 @@ let ounion_get_value
   (ensures (fun _ -> True))
 = gtdata_get_value (Some?.v v) fd
 
-private
 let ounion_create
   (l: union_typ)
   (fd: struct_field l)
@@ -692,7 +362,6 @@ let ounion_create
 : Tot (ounion l)
 = Some (gtdata_create fd v)
 
-private
 let otype_of_typ_union
   (l: union_typ)
 : Lemma
@@ -700,7 +369,6 @@ let otype_of_typ_union
   [SMTPat (otype_of_typ (TUnion l))]
 = assert_norm (otype_of_typ (TUnion l) == ounion l)
 
-private
 let struct_field_is_readable
   (l: struct_typ)
   (ovalue_is_readable: (
@@ -717,7 +385,6 @@ let struct_field_is_readable
   then ovalue_is_readable (typ_of_struct_field l s) (ostruct_sel v s)
   else true
 
-private
 let rec ovalue_is_readable
   (t: typ)
   (v: otype_of_typ t)
@@ -761,7 +428,6 @@ let rec ovalue_is_readable
     let (v: option (buffer t)) = v in
     Some? v
 
-private
 let ovalue_is_readable_struct_intro'
   (l: struct_typ)
   (v: otype_of_typ (TStruct l))
@@ -774,7 +440,6 @@ let ovalue_is_readable_struct_intro'
   (ensures (ovalue_is_readable (TStruct l) v))
 = assert_norm (ovalue_is_readable (TStruct l) v == true)
 
-private
 let ovalue_is_readable_struct_intro
   (l: struct_typ)
   (v: otype_of_typ (TStruct l))
@@ -789,7 +454,6 @@ let ovalue_is_readable_struct_intro
 = List.Tot.for_all_mem (struct_field_is_readable l ovalue_is_readable v) (List.Tot.map fst l);
   ovalue_is_readable_struct_intro' l v
 
-private
 let rec ovalue_is_readable_struct_elim
   (l: struct_typ)
   (v: otype_of_typ (TStruct l))
@@ -808,7 +472,6 @@ let rec ovalue_is_readable_struct_elim
   List.Tot.for_all_mem (struct_field_is_readable l ovalue_is_readable v) (List.Tot.map fst l);
   assert (ovalue_is_readable (typ_of_struct_field l fd) (ostruct_sel v fd))
 
-private
 let ovalue_is_readable_array_elim
   (#len: array_length_t )
   (#t: typ)
@@ -824,7 +487,6 @@ let ovalue_is_readable_array_elim
   [SMTPat (ovalue_is_readable t (Seq.index (Some?.v v) (UInt32.v i)))]
 = ()
 
-private
 let ovalue_is_readable_array_intro
   (#len: array_length_t )
   (#t: typ)
@@ -848,7 +510,6 @@ let ovalue_is_readable_array_intro
   in
   Classical.forall_intro f
 
-private
 let ostruct_field_of_struct_field
   (l: struct_typ)
   (ovalue_of_value: (
@@ -863,7 +524,6 @@ let ostruct_field_of_struct_field
 : Tot (otype_of_struct_field l f)
 = ovalue_of_value (typ_of_struct_field l f) (struct_sel #l v f)
 
-private
 let rec ovalue_of_value
   (t: typ)
   (v: type_of_typ t)
@@ -896,7 +556,6 @@ let rec ovalue_of_value
     ounion_create l k (ovalue_of_value (typ_of_struct_field l k) (union_get_value v k))
   | _ -> Some v
 
-private
 let ovalue_is_readable_ostruct_field_of_struct_field
   (l: struct_typ)
   (ih: (
@@ -912,7 +571,6 @@ let ovalue_is_readable_ostruct_field_of_struct_field
   (ovalue_is_readable (typ_of_struct_field l f) (ostruct_field_of_struct_field l ovalue_of_value v f))
 = ih (typ_of_struct_field l f) (struct_sel #l v f)
 
-private
 let rec ovalue_is_readable_ovalue_of_value
   (t: typ)
   (v: type_of_typ t)
@@ -952,7 +610,6 @@ let rec ovalue_is_readable_ovalue_of_value
     ovalue_is_readable_ovalue_of_value (typ_of_struct_field l k) (union_get_value v k)
   | _ -> ()
 
-private
 let rec value_of_ovalue
   (t: typ)
   (v: otype_of_typ t)
@@ -1017,7 +674,6 @@ let rec value_of_ovalue
 
 #reset-options "--z3rlimit 16"
 
-private
 let rec value_of_ovalue_of_value
   (t: typ)
   (v: type_of_typ t)
@@ -1054,7 +710,6 @@ let rec value_of_ovalue_of_value
     value_of_ovalue_of_value (typ_of_struct_field l k) (union_get_value v k)
   | _ -> ()
 
-private
 let none_ovalue
   (t: typ)
 : Tot (otype_of_typ t)
@@ -1067,7 +722,6 @@ let none_ovalue
   | TNPointer t' -> (None <: option (npointer t'))
   | TBuffer t' -> (None <: option (buffer t'))
 
-private
 let not_ovalue_is_readable_none_ovalue
   (t: typ)
 : Lemma
@@ -1078,7 +732,6 @@ let not_ovalue_is_readable_none_ovalue
 
 (** Pointer paths *)
 
-private
 let step_sel
   (#from: typ)
   (#to: typ)
@@ -1109,7 +762,6 @@ let step_sel
 
 (* TODO: we used to have this:
 <<<
-private
 let ovalue_is_readable_step_sel
   (#from: typ)
   (#to: typ)
@@ -1126,7 +778,6 @@ let ovalue_is_readable_step_sel
 Which is, of course, wrong with unions. So we have to specialize this rule for each step:
 *)
 
-private
 let ovalue_is_readable_step_sel_cell
   (#length: array_length_t)
   (#value: typ)
@@ -1138,7 +789,6 @@ let ovalue_is_readable_step_sel_cell
   [SMTPat (ovalue_is_readable value (step_sel m' (StepCell length value index)))]
 = ()
 
-private
 let ovalue_is_readable_step_sel_field
   (#l: struct_typ)
   (m: ostruct l)
@@ -1149,7 +799,6 @@ let ovalue_is_readable_step_sel_field
   [SMTPat (ovalue_is_readable (typ_of_struct_field l fd) (step_sel m (StepField l fd)))]
 = ()
 
-private
 let ovalue_is_readable_step_sel_union_same
   (#l: union_typ)
   (m: ounion l)
@@ -1162,7 +811,6 @@ let ovalue_is_readable_step_sel_union_same
   (ensures (ovalue_is_readable (typ_of_struct_field l fd) (step_sel m (StepUField l fd))))
 = ()
 
-private
 let step_sel_none_ovalue
   (#from: typ)
   (#to: typ)
@@ -1171,7 +819,7 @@ let step_sel_none_ovalue
   (step_sel (none_ovalue from) s == none_ovalue to)
 = ()
 
-private let rec path_sel
+let rec path_sel
   (#from: typ)
   (#to: typ)
   (m: otype_of_typ from)
@@ -1184,7 +832,6 @@ private let rec path_sel
     let (m': otype_of_typ through') = path_sel m p' in
     step_sel m' s
 
-private
 let rec path_sel_none_ovalue
   (#from: typ)
   (#to: typ)
@@ -1198,7 +845,6 @@ let rec path_sel_none_ovalue
   | PathStep through' to' p' s ->
     path_sel_none_ovalue p'
 
-private
 let step_upd
   (#from: typ)
   (#to: typ)
@@ -1253,7 +899,6 @@ let step_upd
     (* overwrite the whole union with the new field *)
     ounion_create l fd v
 
-private
 let step_sel_upd_same
   (#from: typ)
   (#to: typ)
@@ -1264,7 +909,7 @@ let step_sel_upd_same
   (step_sel (step_upd m s v) s == v)
 = ()
 
-private let rec path_upd
+let rec path_upd
   (#from: typ)
   (#to: typ)
   (m: otype_of_typ from)
@@ -1278,7 +923,7 @@ private let rec path_upd
     let s = path_sel m p' in
     path_upd m p' (step_upd s st v)
 
-private let rec path_sel_upd_same
+let rec path_sel_upd_same
   (#from: typ)
   (#to: typ)
   (m: otype_of_typ from)
@@ -1297,7 +942,7 @@ private let rec path_sel_upd_same
     let s' = step_upd s st v in
     path_sel_upd_same m p' s'
 
-private let rec path_concat
+let rec path_concat
   (#from: typ)
   (#through: typ)
   (#to: typ)
@@ -1311,7 +956,7 @@ private let rec path_concat
   | PathBase -> p
   | PathStep through' to' q' st -> PathStep through' to' (path_concat p q') st
 
-private let path_concat_base_r
+let path_concat_base_r
   (#from: typ)
   (#to: typ)
   (p: path from to)
@@ -1319,7 +964,7 @@ private let path_concat_base_r
   (ensures (path_concat p PathBase == p))
 = ()
 
-private let rec path_concat_base_l
+let rec path_concat_base_l
   (#from: typ)
   (#to: typ)
   (p: path from to)
@@ -1332,7 +977,7 @@ private let rec path_concat_base_l
   | PathBase -> ()
   | PathStep _ _ p' _ -> path_concat_base_l p'
 
-private let rec path_concat_assoc
+let rec path_concat_assoc
   (#t0 #t1 #t2 #t3: typ)
   (p01: path t0 t1)
   (p12: path t1 t2)
@@ -1345,7 +990,7 @@ private let rec path_concat_assoc
   | PathBase -> ()
   | PathStep _ _ p23' _ -> path_concat_assoc p01 p12 p23'
 
-private let rec path_sel_concat
+let rec path_sel_concat
   (#from: typ)
   (#through: typ)
   (#to: typ)
@@ -1361,7 +1006,7 @@ private let rec path_sel_concat
   | PathBase -> ()
   | PathStep _ _ q' _ -> path_sel_concat m p q'
 
-private let rec path_upd_concat
+let rec path_upd_concat
   (#from: typ)
   (#through: typ)
   (#to: typ)
@@ -1382,7 +1027,7 @@ private let rec path_upd_concat
     path_upd_concat m p q' s'
 
 // TODO: rename as: prefix_of; use infix notation (p1 `prefix_of` p2)
-private let rec path_includes
+let rec path_includes
   (#from: typ)
   (#to1 #to2: typ)
   (p1: path from to1)
@@ -1397,7 +1042,7 @@ private let rec path_includes
     path_includes p1 p2'
   )
 
-private let rec path_includes_base
+let rec path_includes_base
   (#from: typ)
   (#to: typ)
   (p: path from to)
@@ -1410,7 +1055,7 @@ private let rec path_includes_base
   | PathBase -> ()
   | PathStep _ _ p2' _ -> path_includes_base p2'
 
-private let path_includes_refl
+let path_includes_refl
   (#from #to: typ)
   (p: path from to)
 : Lemma
@@ -1419,7 +1064,7 @@ private let path_includes_refl
   [SMTPat (path_includes p p)]
 = ()
 
-private let path_includes_step_r
+let path_includes_step_r
   (#from #through #to: typ)
   (p: path from through)
   (s: step through to)
@@ -1429,7 +1074,7 @@ private let path_includes_step_r
   [SMTPat (path_includes p (PathStep through to p s))]
 = ()
 
-private let rec path_includes_trans
+let rec path_includes_trans
   (#from #to1 #to2 #to3: typ)
   (p1: path from to1)
   (p2: path from to2)
@@ -1452,7 +1097,7 @@ private let rec path_includes_trans
 	path_includes_trans p1 p2 p3'
     )
 
-private let rec path_includes_ind
+let rec path_includes_ind
   (#from: typ)
   (x: (#to1: typ) ->
       (#to2: typ) ->
@@ -1501,7 +1146,7 @@ private let rec path_includes_ind
        h_trans p1 p2' p2
     )
 
-private let rec path_length
+let rec path_length
   (#from #to: typ)
   (p: path from to)
 : Tot nat
@@ -1510,7 +1155,7 @@ private let rec path_length
   | PathBase -> 0
   | PathStep _ _ p' _ -> 1 + path_length p'
 
-private let path_includes_length
+let path_includes_length
   (#from: typ)
   (#to1 #to2: typ)
   (p1: path from to1)
@@ -1524,7 +1169,7 @@ private let path_includes_length
     (fun #to1_ #to2_ #to3_ p1_ p2_ p3_ -> ())
     p1 p2
 
-private let path_includes_step_l
+let path_includes_step_l
   (#from: typ)
   (#through: typ)
   (#to: typ)
@@ -1537,7 +1182,7 @@ private let path_includes_step_l
 = assert (path_length (PathStep through to p s) > path_length p);
   FStar.Classical.forall_intro (path_includes_length #from #to #through (PathStep through to p s))
 
-private let rec path_includes_concat
+let rec path_includes_concat
   (#from: typ)
   (#through: typ)
   (#to: typ)
@@ -1552,7 +1197,7 @@ private let rec path_includes_concat
   | PathBase -> ()
   | PathStep _ _ q' _ -> path_includes_concat p q'
 
-private let path_includes_exists_concat
+let path_includes_exists_concat
   (#from #through: typ)
   (p: path from through)
   (#to: typ)
@@ -1573,7 +1218,7 @@ private let path_includes_exists_concat
     )
     p q
 
-private let path_concat_includes
+let path_concat_includes
   (#from #through: typ)
   (p: path from through)
   (phi: (
@@ -1597,7 +1242,6 @@ private let path_concat_includes
 = Classical.forall_intro_2 f;
   path_includes_exists_concat p q
 
-private
 let step_disjoint
   (#from: typ)
   (#to1 #to2: typ)
@@ -1615,7 +1259,6 @@ let step_disjoint
     (* two fields of the same union are never disjoint *)
     false
 
-private
 let step_eq
   (#from: typ)
   (#to1 #to2: typ)
@@ -1633,7 +1276,6 @@ let step_eq
     let (StepUField _ fd2) = s2 in
     fd1 = fd2
 
-private
 let step_disjoint_not_eq
   (#from: typ)
   (#to1 #to2: typ)
@@ -1644,7 +1286,6 @@ let step_disjoint_not_eq
   (ensures (step_eq s1 s2 == false))
 = () (* Note: the converse is now wrong, due to unions *)
 
-private
 let step_disjoint_sym
   (#from: typ)
   (#to1 #to2: typ)
@@ -1655,7 +1296,7 @@ let step_disjoint_sym
   (ensures (step_disjoint s2 s1))
 = ()
 
-noeq private type path_disjoint_t (#from: typ):
+noeq type path_disjoint_t (#from: typ):
   (#to1: typ) ->
   (#to2: typ) ->
   (p1: path from to1) ->
@@ -1681,7 +1322,7 @@ noeq private type path_disjoint_t (#from: typ):
     path_disjoint_t p1 p2 ->
     path_disjoint_t p1' p2'
 
-private let rec path_disjoint_t_rect
+let rec path_disjoint_t_rect
   (#from: typ)
   (x:
     (#value1: typ) ->
@@ -1725,7 +1366,7 @@ private let rec path_disjoint_t_rect
   | PathDisjointStep p s1 s2 -> h_step p s1 s2 h
   | PathDisjointIncludes p1_ p2_ p1' p2' h_ -> h_includes p1_ p2_ p1' p2' h_ h (path_disjoint_t_rect x h_step h_includes p1_ p2_ h_)
 
-private let path_disjoint
+let path_disjoint
   (#from: typ)
   (#value1: typ)
   (#value2: typ)
@@ -1734,7 +1375,7 @@ private let path_disjoint
 : GTot Type0
 = squash (path_disjoint_t p1 p2)
 
-private let path_disjoint_ind
+let path_disjoint_ind
   (#from: typ)
   (x:
     (#value1: typ) ->
@@ -1777,7 +1418,7 @@ private let path_disjoint_ind
        h_includes p1 p2 p1' p2')
      p1 p2 h)
 
-private let path_disjoint_step
+let path_disjoint_step
   (#from: typ)
   (#through: typ)
   (#to1: typ)
@@ -1791,7 +1432,7 @@ private let path_disjoint_step
   [SMTPat (path_disjoint (PathStep through to1 p s1) (PathStep through to2 p s2))]
 = FStar.Squash.return_squash (PathDisjointStep p s1 s2)
 
-private let path_disjoint_includes
+let path_disjoint_includes
   (#from: typ)
   (#to1: typ)
   (#to2: typ)
@@ -1806,7 +1447,6 @@ private let path_disjoint_includes
 = let h : squash (path_disjoint_t p1 p2) = FStar.Squash.join_squash () in
   FStar.Squash.bind_squash h (fun h -> FStar.Squash.return_squash (PathDisjointIncludes p1 p2 p1' p2' h))
 
-private
 let rec path_disjoint_sym
   (#from: typ)
   (#value1: typ)
@@ -1822,7 +1462,7 @@ let rec path_disjoint_sym
   (fun #v1 #v2 p1 p2 #v1' #v2' p1' p2' -> path_disjoint_includes p2 p1 p2' p1')
   p1 p2
 
-private let rec path_equal
+let rec path_equal
   (#from: typ)
   (#value1: typ)
   (#value2: typ)
@@ -1839,7 +1479,6 @@ private let rec path_equal
         step_eq s1 s2
     ))
 
-private
 let rec path_length_concat
   (#t0 #t1 #t2: typ)
   (p01: path t0 t1)
@@ -1852,7 +1491,6 @@ let rec path_length_concat
   | PathBase -> ()
   | PathStep _ _ p' s' -> path_length_concat p01 p'
 
-private
 let rec path_concat_inj_l
   (#from #through1: typ)
   (p1_: path from through1)
@@ -1873,7 +1511,7 @@ let rec path_concat_inj_l
     let (PathStep _ _ p2' s2) = p2 in
     path_concat_inj_l p1_ p1' p2_ p2'
 
-private type path_disjoint_decomp_t
+type path_disjoint_decomp_t
   (#from: typ)
   (#value1: typ)
   (#value2: typ)
@@ -1896,7 +1534,7 @@ private type path_disjoint_decomp_t
     ) ->
     path_disjoint_decomp_t p1 p2
 
-private let path_disjoint_decomp_includes
+let path_disjoint_decomp_includes
   (#from: typ)
   (#value1: typ)
   (#value2: typ)
@@ -1951,7 +1589,6 @@ private let path_disjoint_decomp_includes
   in
   ()
 
-private
 let path_disjoint_decomp
   (#from: typ)
   (#value1: typ)
@@ -1972,7 +1609,6 @@ let path_disjoint_decomp
   (fun #v1 #v2 p1 p2 #v1' #v2' p1' p2' -> path_disjoint_decomp_includes p1 p2 p1' p2')
   p1 p2
 
-private
 let path_disjoint_not_path_equal
   (#from: typ)
   (#value1: typ)
@@ -1994,7 +1630,6 @@ let path_disjoint_not_path_equal
   path_disjoint_decomp p1 p2;
   Classical.forall_intro f
 
-private
 let rec path_destruct_l
   (#t0 #t2: typ)
   (p: path t0 t2)
@@ -2012,7 +1647,6 @@ let rec path_destruct_l
       Some (| t_, (| s_, PathStep _ _ p_ s |) |)
     end
 
-private
 let rec path_equal'
   (#from #to1 #to2: typ)
   (p1: path from to1)
@@ -2029,7 +1663,6 @@ let rec path_equal'
       path_equal' p1' p2'
     end
 
-private
 let path_includes_concat_l
   (#from #through #to1 #to2: typ)
   (p0: path from through)
@@ -2045,7 +1678,6 @@ let path_includes_concat_l
     (fun #to1_ #to2_ #to3_ p1_ p2_ p3_ -> path_includes_trans (path_concat p0 p1_) (path_concat p0 p2_) (path_concat p0 p3_))
     p1 p2
 
-private
 let path_disjoint_concat
   (#from #through #to1 #to2: typ)
   (p0: path from through)
@@ -2064,7 +1696,6 @@ let path_disjoint_concat
   p1 p2
 
 (* TODO: the following is now wrong due to unions, but should still hold if we restrict ourselves to readable paths
-private
 let rec not_path_equal_path_disjoint_same_type
   (#from: typ)
   (#value: typ)
@@ -2094,7 +1725,6 @@ let rec not_path_equal_path_disjoint_same_type
     end
 *)
 
-private
 let step_sel_upd_other
   (#from: typ)
   (#to1 #to2: typ)
@@ -2121,7 +1751,7 @@ let step_sel_upd_other
       Seq.lemma_index_upd2 m (UInt32.v i1) v (UInt32.v i2)
     end
 
-private let path_sel_upd_other
+let path_sel_upd_other
   (#from: typ)
   (#to1 #to2: typ)
   (p1: path from to1)
@@ -2152,7 +1782,7 @@ private let path_sel_upd_other
 	  )))))
   p1 p2
 
-private let path_sel_upd_other'
+let path_sel_upd_other'
   (#from: typ)
   (#to1 #to2: typ)
   (p1: path from to1)
@@ -2167,7 +1797,7 @@ private let path_sel_upd_other'
 
 (** Operations on pointers *)
 
-abstract let equal
+let equal
   (#t1 #t2: typ)
   (p1: pointer t1)
   (p2: pointer t2)
@@ -2178,10 +1808,10 @@ abstract let equal
   HS.aref_equal (Pointer?.contents p1) (Pointer?.contents p2) &&
   path_equal (Pointer?.p p1) (Pointer?.p p2)
 
-abstract let as_addr (#t: typ) (p: pointer t): GTot nat =
+let as_addr (#t: typ) (p: pointer t): GTot nat =
   HS.aref_as_addr (Pointer?.contents p)
 
-private let _field
+let _field
   (#l: struct_typ)
   (p: pointer (TStruct l))
   (fd: struct_field l)
@@ -2191,7 +1821,7 @@ private let _field
   let p'' : path from (typ_of_struct_field l fd) = PathStep _ _ p' (StepField _ fd) in
   Pointer from contents p''
 
-private let _cell
+let _cell
   (#length: array_length_t)
   (#value: typ)
   (p: pointer (TArray length value))
@@ -2202,7 +1832,7 @@ private let _cell
   let p'' : path from value = PathStep _ _ p' (StepCell _ _ i) in
   Pointer from contents p''
 
-private let _ufield
+let _ufield
   (#l: union_typ)
   (p: pointer (TUnion l))
   (fd: struct_field l)
@@ -2212,7 +1842,7 @@ private let _ufield
   let p'' : path from (typ_of_struct_field l fd) = PathStep _ _ p' (StepUField _ fd) in
   Pointer from contents p''
 
-abstract let unused_in
+let unused_in
   (#value: typ)
   (p: pointer value)
   (h: HS.mem)
@@ -2220,10 +1850,9 @@ abstract let unused_in
 = let (Pointer from contents p') = p in
   HS.aref_unused_in contents h
 
-private
 let pointer_ref_contents : Type0 = (t: typ & otype_of_typ t)
 
-abstract let live
+let live
   (#value: typ)
   (h: HS.mem)
   (p: pointer value)
@@ -2235,7 +1864,6 @@ abstract let live
       dfst (HS.sel h untyped_contents) == from
   )))
 
-abstract
 let nlive
   (#value: typ)
   (h: HS.mem)
@@ -2245,7 +1873,6 @@ let nlive
   then True
   else live h p
 
-abstract
 let live_nlive
   (#value: typ)
   (h: HS.mem)
@@ -2255,7 +1882,6 @@ let live_nlive
   [SMTPat (nlive h p)]
 = ()
 
-abstract
 let g_is_null_nlive
   (#t: typ)
   (h: HS.mem)
@@ -2266,7 +1892,7 @@ let g_is_null_nlive
   [SMTPat (g_is_null p); SMTPat (nlive h p)]
 = ()
 
-private let greference_of
+let greference_of
   (#value: typ)
   (p: pointer value)
 : Ghost (HS.reference pointer_ref_contents)
@@ -2274,7 +1900,6 @@ private let greference_of
   (ensures (fun x -> (exists h . live h p) /\ x == HS.greference_of (Pointer?.contents p) pointer_ref_contents (Heap.trivial_preorder pointer_ref_contents) /\ HS.aref_of x == Pointer?.contents p))
 = HS.greference_of (Pointer?.contents p) pointer_ref_contents (Heap.trivial_preorder pointer_ref_contents)
 
-private
 let unused_in_greference_of
   (#value: typ)
   (p: pointer value)
@@ -2288,7 +1913,7 @@ let unused_in_greference_of
   ]]
 = ()
 
-abstract let live_not_unused_in
+let live_not_unused_in
   (#value: typ)
   (h: HS.mem)
   (p: pointer value)
@@ -2303,7 +1928,7 @@ abstract let live_not_unused_in
   in
   Classical.move_requires f ()
 
-abstract let gread
+let gread
   (#value: typ)
   (h: HS.mem)
   (p: pointer value)
@@ -2316,13 +1941,13 @@ abstract let gread
   else
     dummy_val value
 
-abstract let frameOf
+let frameOf
   (#value: typ)
   (p: pointer value)
 : GTot HH.rid
 = HS.frameOf_aref (Pointer?.contents p)
 
-abstract let disjoint_roots_intro_pointer_vs_pointer
+let disjoint_roots_intro_pointer_vs_pointer
   (#value1 value2: typ)
   (h: HS.mem)
   (p1: pointer value1)
@@ -2332,7 +1957,7 @@ abstract let disjoint_roots_intro_pointer_vs_pointer
   (ensures (frameOf p1 <> frameOf p2 \/ as_addr p1 =!= as_addr p2))
 = ()
 
-abstract let disjoint_roots_intro_pointer_vs_reference
+let disjoint_roots_intro_pointer_vs_reference
   (#value1: typ)
   (#value2: Type)
   (h: HS.mem)
@@ -2343,7 +1968,7 @@ abstract let disjoint_roots_intro_pointer_vs_reference
   (ensures (frameOf p1 <> HS.frameOf p2 \/ as_addr p1 =!= HS.as_addr p2))
 = ()
 
-abstract let disjoint_roots_intro_reference_vs_pointer
+let disjoint_roots_intro_reference_vs_pointer
   (#value1: Type)
   (#value2: typ)
   (h: HS.mem)
@@ -2354,14 +1979,14 @@ abstract let disjoint_roots_intro_reference_vs_pointer
   (ensures (HS.frameOf p1 <> frameOf p2 \/ HS.as_addr p1 =!= as_addr p2))
 = ()
 
-abstract let is_mm
+let is_mm
   (#value: typ)
   (p: pointer value)
 : GTot bool
 = HS.aref_is_mm (Pointer?.contents p)
 
 (* // TODO: recover with addresses?
-abstract let recall
+let recall
   (#value: Type)
   (p: pointer value {HS.is_eternal_region (frameOf p) && not (is_mm p)})
 : HST.Stack unit
@@ -2370,7 +1995,7 @@ abstract let recall
 = HST.recall (Pointer?.content p)
 *)
 
-abstract let includes
+let includes
   (#value1: typ)
   (#value2: typ)
   (p1: pointer value1)
@@ -2382,14 +2007,14 @@ abstract let includes
 
 #reset-options "--z3rlimit 16"
 
-abstract let gfield
+let gfield
   (#l: struct_typ)
   (p: pointer (TStruct l))
   (fd: struct_field l)
 : GTot (p' : pointer (typ_of_struct_field l fd) { includes p p' } )
 = _field p fd
 
-abstract let as_addr_gfield
+let as_addr_gfield
   (#l: struct_typ)
   (p: pointer (TStruct l))
   (fd: struct_field l)
@@ -2399,7 +2024,7 @@ abstract let as_addr_gfield
   [SMTPat (as_addr (gfield p fd))]
 = ()
 
-abstract let unused_in_gfield
+let unused_in_gfield
   (#l: struct_typ)
   (p: pointer (TStruct l))
   (fd: struct_field l)
@@ -2410,7 +2035,7 @@ abstract let unused_in_gfield
   [SMTPat (unused_in (gfield p fd) h)]
 = ()
 
-abstract let live_gfield
+let live_gfield
   (h: HS.mem)
   (#l: struct_typ)
   (p: pointer (TStruct l))
@@ -2421,7 +2046,7 @@ abstract let live_gfield
   [SMTPat (live h (gfield p fd))]
 = ()
 
-abstract let gread_gfield
+let gread_gfield
   (h: HS.mem)
   (#l: struct_typ)
   (p: pointer (TStruct l))
@@ -2432,7 +2057,7 @@ abstract let gread_gfield
   [SMTPatOr [[SMTPat (gread h (gfield p fd))]; [SMTPat (struct_sel (gread h p) fd)]]]
 = ()
 
-abstract let frameOf_gfield
+let frameOf_gfield
   (#l: struct_typ)
   (p: pointer (TStruct l))
   (fd: struct_field l)
@@ -2442,7 +2067,7 @@ abstract let frameOf_gfield
   [SMTPat (frameOf (gfield p fd))]
 = ()
 
-abstract let is_mm_gfield
+let is_mm_gfield
   (#l: struct_typ)
   (p: pointer (TStruct l))
   (fd: struct_field l)
@@ -2452,7 +2077,7 @@ abstract let is_mm_gfield
   [SMTPat (is_mm (gfield p fd))]
 = ()
 
-abstract let includes_gfield
+let includes_gfield
   (#l: struct_typ)
   (p: pointer (TStruct l))
   (fd: struct_field l)
@@ -2462,14 +2087,14 @@ abstract let includes_gfield
   [SMTPat (includes p (gfield p fd))]
 = ()
 
-abstract let gufield
+let gufield
   (#l: union_typ)
   (p: pointer (TUnion l))
   (fd: struct_field l)
 : GTot (p' : pointer (typ_of_struct_field l fd) { includes p p' } )
 = _ufield p fd
 
-abstract let as_addr_gufield
+let as_addr_gufield
   (#l: union_typ)
   (p: pointer (TUnion l))
   (fd: struct_field l)
@@ -2479,7 +2104,7 @@ abstract let as_addr_gufield
   [SMTPat (as_addr (gufield p fd))]
 = ()
 
-abstract let unused_in_gufield
+let unused_in_gufield
   (#l: union_typ)
   (p: pointer (TUnion l))
   (fd: struct_field l)
@@ -2490,7 +2115,7 @@ abstract let unused_in_gufield
   [SMTPat (unused_in (gufield p fd) h)]
 = ()
 
-abstract let live_gufield
+let live_gufield
   (h: HS.mem)
   (#l: union_typ)
   (p: pointer (TUnion l))
@@ -2501,7 +2126,7 @@ abstract let live_gufield
   [SMTPat (live h (gufield p fd))]
 = ()
 
-abstract let gread_gufield
+let gread_gufield
   (h: HS.mem)
   (#l: union_typ)
   (p: pointer (TUnion l))
@@ -2515,7 +2140,7 @@ abstract let gread_gufield
   [SMTPatOr [[SMTPat (gread h (gufield p fd))]; [SMTPat (union_get_value (gread h p) fd)]]]
 = ()
 
-abstract let frameOf_gufield
+let frameOf_gufield
   (#l: union_typ)
   (p: pointer (TUnion l))
   (fd: struct_field l)
@@ -2525,7 +2150,7 @@ abstract let frameOf_gufield
   [SMTPat (frameOf (gufield p fd))]
 = ()
 
-abstract let is_mm_gufield
+let is_mm_gufield
   (#l: union_typ)
   (p: pointer (TUnion l))
   (fd: struct_field l)
@@ -2535,7 +2160,7 @@ abstract let is_mm_gufield
   [SMTPat (is_mm (gufield p fd))]
 = ()
 
-abstract let includes_gufield
+let includes_gufield
   (#l: union_typ)
   (p: pointer (TUnion l))
   (fd: struct_field l)
@@ -2545,7 +2170,7 @@ abstract let includes_gufield
   [SMTPat (includes p (gufield p fd))]
 = ()
 
-abstract let gcell
+let gcell
   (#length: array_length_t)
   (#value: typ)
   (p: pointer (TArray length value))
@@ -2553,7 +2178,7 @@ abstract let gcell
 : GTot (pointer value)
 = _cell p i
 
-abstract let as_addr_gcell
+let as_addr_gcell
   (#length: array_length_t)
   (#value: typ)
   (p: pointer (TArray length value))
@@ -2564,7 +2189,7 @@ abstract let as_addr_gcell
   [SMTPat (as_addr (gcell p i))]
 = ()
 
-abstract let unused_in_gcell
+let unused_in_gcell
   (#length: array_length_t)
   (#value: typ)
   (h: HS.mem)
@@ -2576,7 +2201,7 @@ abstract let unused_in_gcell
   [SMTPat (unused_in (gcell p i) h)]
 = ()
 
-abstract let live_gcell
+let live_gcell
   (#length: array_length_t)
   (#value: typ)
   (h: HS.mem)
@@ -2588,7 +2213,7 @@ abstract let live_gcell
   [SMTPat (live h (gcell p i))]
 = ()
 
-abstract let gread_gcell
+let gread_gcell
   (#length: array_length_t)
   (#value: typ)
   (h: HS.mem)
@@ -2600,7 +2225,7 @@ abstract let gread_gcell
   [SMTPat (gread h (gcell p i))]
 = ()
 
-abstract let frameOf_gcell
+let frameOf_gcell
   (#length: array_length_t)
   (#value: typ)
   (p: pointer (TArray length value))
@@ -2611,7 +2236,7 @@ abstract let frameOf_gcell
   [SMTPat (frameOf (gcell p i))]
 = ()
 
-abstract let is_mm_gcell
+let is_mm_gcell
   (#length: array_length_t)
   (#value: typ)
   (p: pointer (TArray length value))
@@ -2622,7 +2247,7 @@ abstract let is_mm_gcell
   [SMTPat (is_mm (gcell p i))]
 = ()
 
-abstract let includes_gcell
+let includes_gcell
   (#length: array_length_t)
   (#value: typ)
   (p: pointer (TArray length value))
@@ -2633,7 +2258,7 @@ abstract let includes_gcell
   [SMTPat (includes p (gcell p i))]
 = ()
 
-abstract let includes_refl
+let includes_refl
   (#value: typ)
   (p: pointer value)
 : Lemma
@@ -2642,7 +2267,7 @@ abstract let includes_refl
   [SMTPat (includes p p)]
 = ()
 
-abstract let includes_trans
+let includes_trans
   (#value1 #value2 #value3: typ)
   (p1: pointer value1)
   (p2: pointer value2)
@@ -2653,7 +2278,7 @@ abstract let includes_trans
   [SMTPatT (includes p1 p2); SMTPatT (includes p2 p3)]
 = path_includes_trans (Pointer?.p p1) (Pointer?.p p2) (Pointer?.p p3)
 
-abstract let includes_ind
+let includes_ind
   (x: (#value1: typ) ->
       (#value2: typ) ->
       (p1: pointer value1) ->
@@ -2706,7 +2331,6 @@ abstract let includes_ind
     (Pointer?.p p1)
     (Pointer?.p p2)
 
-abstract
 let unused_in_includes
   (#value1: typ)
   (#value2: typ)
@@ -2726,7 +2350,6 @@ let unused_in_includes
   (fun #v1 #v2 #v3 p1 p2 p3 -> ())
   p1 p2
 
-abstract
 let live_includes
   (#value1: typ)
   (#value2: typ)
@@ -2746,7 +2369,7 @@ let live_includes
   (fun #v1 #v2 #v3 p1 p2 p3 -> ())
   p1 p2
 
-abstract let disjoint
+let disjoint
   (#value1: typ)
   (#value2: typ)
   (p1: pointer value1)
@@ -2762,7 +2385,7 @@ abstract let disjoint
   else
     True
 
-abstract let disjoint_root
+let disjoint_root
   (#value1: typ)
   (#value2: typ)
   (p1: pointer value1)
@@ -2772,7 +2395,7 @@ abstract let disjoint_root
   (ensures (disjoint p1 p2))
 = ()
 
-abstract let disjoint_gfield
+let disjoint_gfield
   (#l: struct_typ)
   (p: pointer (TStruct l))
   (fd1 fd2: struct_field l)
@@ -2782,7 +2405,7 @@ abstract let disjoint_gfield
   [SMTPat (disjoint (gfield p fd1) (gfield p fd2))]
 = ()
 
-abstract let disjoint_gcell
+let disjoint_gcell
   (#length: array_length_t)
   (#value: typ)
   (p: pointer (TArray length value))
@@ -2794,7 +2417,7 @@ abstract let disjoint_gcell
   [SMTPat (disjoint (gcell p i1) (gcell p i2))]
 = ()
 
-abstract let disjoint_includes
+let disjoint_includes
   (#value1: typ)
   (#value2: typ)
   (p1: pointer value1)
@@ -2814,7 +2437,7 @@ abstract let disjoint_includes
   else
     ()
 
-abstract let disjoint_ind
+let disjoint_ind
   (x:
     (#value1: typ) ->
     (#value2: typ) ->
@@ -2879,7 +2502,6 @@ abstract let disjoint_ind
   else
     h_root p1 p2
 
-abstract
 let disjoint_sym
   (#value1: typ)
   (#value2: typ)
@@ -2896,7 +2518,6 @@ let disjoint_sym
   (fun #v1 #v2 p1 p2 #v1' #v2' p1' p2' -> disjoint_includes p2 p1 p2' p1')
   p1 p2
 
-abstract
 let disjoint_sym'
   (#value1: typ)
   (#value2: typ)
@@ -2909,14 +2530,12 @@ let disjoint_sym'
 = FStar.Classical.move_requires (disjoint_sym #value1 #value2 p1) p2;
   FStar.Classical.move_requires (disjoint_sym #value2 #value1 p2) p1
 
-abstract
 let disjoint_includes_l #a #as #a' (x: pointer a) (subx:pointer as) (y:pointer a') : Lemma
   (requires (includes x subx /\ disjoint x y))
   (ensures  (disjoint subx y))
   [SMTPatT (disjoint subx y); SMTPatT (includes x subx)]
   = disjoint_includes x y subx y
 
-abstract
 let disjoint_includes_l_swap #a #as #a' (x:pointer a) (subx:pointer as) (y:pointer a') : Lemma
   (requires (includes x subx /\ disjoint x y))
   (ensures  (disjoint y subx))
@@ -2925,7 +2544,6 @@ let disjoint_includes_l_swap #a #as #a' (x:pointer a) (subx:pointer as) (y:point
 
 (* TODO: The following is now wrong, should be replaced with readable
 
-abstract
 let live_not_equal_disjoint
   (#t: typ)
   (h: HS.mem)
@@ -2945,7 +2563,6 @@ let live_not_equal_disjoint
     disjoint_root p1 p2
 *)
 
-abstract
 let live_unused_in_disjoint_strong
   (#value1: typ)
   (#value2: typ)
@@ -2957,7 +2574,6 @@ let live_unused_in_disjoint_strong
   (ensures (frameOf p1 <> frameOf p2 \/ as_addr p1 <> as_addr p2))
 = ()
 
-abstract
 let live_unused_in_disjoint
   (#value1: typ)
   (#value2: typ)
@@ -2976,19 +2592,18 @@ let live_unused_in_disjoint
     tracking the permission in the heap.
 *)
 
-abstract
 let readable
   (#a: typ)
   (h: HS.mem)
   (b: pointer a)
 : GTot Type0
-= live h b /\ (
+= let () = () in // necessary to somehow remove the `logic` qualifier
+  live h b /\ (
     let content = greference_of b in
     let (| _, c |) = HS.sel h content in
     ovalue_is_readable a (path_sel c (Pointer?.p b))
   )
 
-abstract
 let readable_live
   (#a: typ)
   (h: HS.mem)
@@ -3002,7 +2617,6 @@ let readable_live
   ]]
 = ()
 
-abstract
 let readable_gfield
   (#l: struct_typ)
   (h: HS.mem)
@@ -3014,7 +2628,6 @@ let readable_gfield
   [SMTPat (readable h (gfield p fd))]
 = ()
 
-abstract
 let readable_struct
   (#l: struct_typ)
   (h: HS.mem)
@@ -3035,7 +2648,6 @@ let readable_struct
   let (v: ostruct l {Some? v}) = v in
   ovalue_is_readable_struct_intro l v
 
-abstract
 let readable_struct_forall_mem
   (#l: struct_typ)
   (p: pointer (TStruct l))
@@ -3059,7 +2671,6 @@ let readable_struct_forall_mem
   in
   Classical.forall_intro (Classical.move_requires f)
 
-abstract
 let readable_gcell
   (#length: array_length_t)
   (#value: typ)
@@ -3072,7 +2683,6 @@ let readable_gcell
   [SMTPat (readable h (gcell p i))]
 = ()
 
-abstract
 let readable_array
   (#length: array_length_t)
   (#value: typ)
@@ -3092,7 +2702,6 @@ let readable_array
   ovalue_is_readable_array_intro v0
 
 (* TODO: improve on the following interface *)
-abstract
 let readable_gufield
   (#l: union_typ)
   (h: HS.mem)
@@ -3106,14 +2715,14 @@ let readable_gufield
 
 (** The active field of a union *)
 
-abstract
 let is_active_union_field
   (#l: union_typ)
   (h: HS.mem)
   (p: pointer (TUnion l))
   (fd: struct_field l)
 : GTot Type0
-= live h p /\ (
+= let () = () in // necessary to somehow remove the `logic` qualifier
+  live h p /\ (
     let content = greference_of p in
     let (| _, c |) = HS.sel h content in
     let vu : otype_of_typ (TUnion l) = path_sel c (Pointer?.p p) in
@@ -3121,7 +2730,6 @@ let is_active_union_field
     Some? vu /\ gtdata_get_key (Some?.v vu) == fd
   )
 
-abstract
 let is_active_union_live
   (#l: union_typ)
   (h: HS.mem)
@@ -3133,7 +2741,6 @@ let is_active_union_live
   [SMTPat (is_active_union_field h p fd)]
 = ()
 
-abstract
 let is_active_union_field_live
   (#l: union_typ)
   (h: HS.mem)
@@ -3145,7 +2752,6 @@ let is_active_union_field_live
   [SMTPat (is_active_union_field h p fd)]
 = ()
 
-abstract
 let is_active_union_field_eq
   (#l: union_typ)
   (h: HS.mem)
@@ -3157,7 +2763,6 @@ let is_active_union_field_eq
   [SMTPat (is_active_union_field h p fd1); SMTPat (is_active_union_field h p fd2)]
 = ()
 
-abstract
 let is_active_union_field_get_key
   (#l: union_typ)
   (h: HS.mem)
@@ -3169,7 +2774,6 @@ let is_active_union_field_get_key
   [SMTPat (is_active_union_field h p fd)]
 = ()
 
-abstract
 let is_active_union_field_readable
   (#l: union_typ)
   (h: HS.mem)
@@ -3181,7 +2785,6 @@ let is_active_union_field_readable
   [SMTPat (is_active_union_field h p fd); SMTPat (readable h (gufield p fd))]
 = ()
 
-abstract
 let is_active_union_field_includes_readable
   (#l: union_typ)
   (h: HS.mem)
@@ -3218,22 +2821,7 @@ let is_active_union_field_includes_readable
   path_concat_includes pf phi f (Pointer?.p p')
 
 
-(* Equality predicate on struct contents, without quantifiers *)
-let equal_values #a h (b:pointer a) h' (b':pointer a) : GTot Type0 =
-  live h b /\ live h' b' /\ (
-    readable h b ==> (
-      readable h' b' /\
-      gread h b == gread h' b'
-  ))
-
 (*** The modifies clause *)
-
-// private // in fact, we have to expose this type, otherwise unification problems will appear everywhere
-noeq type apointer =
-| APointer:
-  (a: typ) ->
-  (p: pointer a) ->
-  apointer
 
 (** Sets of pointers. The set tracks not only the set of pointers, but
 also the corresponding set of addresses (which cannot be constructed
@@ -3247,45 +2835,36 @@ We could also completely remove this "assumption" and explicitly track
 the regions and addresses within those regions. But this way would
 actually defeat the practical purpose of regions.
 *)
-private
 let set_addrs_t (pointers : TSet.set apointer) =
   addrs:Set.set nat {
     forall (n: nat) .
       Set.mem n addrs <==>
       (exists (x: apointer) . TSet.mem x pointers /\ as_addr (APointer?.p x) == n) }
 
-abstract
-noeq type set =
+noeq type set' =
 | Set:
   (pointers: TSet.set apointer) ->
   (addrs: Ghost.erased (set_addrs_t pointers) ) ->
-  set
+  set'
+let set = set'
 
-abstract
 let set_amem
   (a: apointer)
   (s: set)
 : GTot Type0
 = TSet.mem a (Set?.pointers s)
 
-let set_mem
-  (#a: typ)
-  (p: pointer a)
-  (s: set)
-: GTot Type0
-= set_amem (APointer a p) s
-
-abstract let set_empty: set =
+let set_empty: set =
   Set TSet.empty (Ghost.hide Set.empty)
 
-abstract let set_amem_empty
+let set_amem_empty
   (x: apointer)
 : Lemma
   (~ (set_amem x set_empty))
   [SMTPat (set_amem x set_empty)]
 = ()
 
-abstract let set_singleton
+let set_singleton
   (#a: typ)
   (x: pointer a)
 : Tot set
@@ -3294,7 +2873,7 @@ abstract let set_singleton
   let f () : GTot (set_addrs_t pointers) = Set.singleton (as_addr x) in
   Set pointers (Ghost.elift1 f (Ghost.hide ()))
 
-abstract let set_amem_singleton
+let set_amem_singleton
   (#a: typ)
   (x: pointer a)
   (x': apointer)
@@ -3303,7 +2882,7 @@ abstract let set_amem_singleton
   [SMTPat (set_amem x' (set_singleton x))]
 = ()
 
-abstract let set_union
+let set_union
   (s1 s2: set)
 : Tot set
 = let pointers = TSet.union (Set?.pointers s1) (Set?.pointers s2) in
@@ -3313,7 +2892,7 @@ abstract let set_union
   in
   Set pointers (Ghost.elift2 union (Set?.addrs s1) (Set?.addrs s2))
 
-abstract let set_amem_union
+let set_amem_union
   (x: apointer)
   (s1 s2: set)
 : Lemma
@@ -3321,17 +2900,6 @@ abstract let set_amem_union
   [SMTPat (set_amem x (set_union s1 s2))]
 = ()
 
-let set_subset
-  (s1 s2: set)
-: Tot Type0
-= forall (x: apointer) . set_amem x s1 ==> set_amem x s2
-
-let set_equal
-  (s1 s2: set)
-: Tot Type0
-= set_subset s1 s2 /\ set_subset s2 s1
-
-abstract
 let set_equal_elim
   (s1 s2: set)
 : Lemma
@@ -3361,6 +2929,16 @@ let set_equal_elim
   in
   ()
 
+let set_includes_singleton
+  (#a1: typ)
+  (p1: pointer a1)
+  (#a2: typ)
+  (p2: pointer a2)
+: Lemma
+  (requires (p1 `includes` p2))
+  (ensures (set_singleton p1 `set_includes` set_singleton p2))
+= ()
+
 (** NOTE: intersection cannot be easily defined, indeed consider two
 different (not necessarily disjoint) pointers p1, p2 coming from the
 same root address, intersect (singleton p1) (singleton p2) will be
@@ -3378,68 +2956,31 @@ modifies clauses.
 
 *)
 
-(** Pointer inclusion lifted to sets of pointers *)
-
-let set_includes
-  (s1 s2: set)
-: GTot Type0
-= forall (ap2: apointer { set_amem ap2 s2 } ) .
-  exists (ap1: apointer { set_amem ap1 s1 } ) .
-  (APointer?.p ap1) `includes` (APointer?.p ap2)
-
-let set_includes_refl
-  (s: set)
-: Lemma
-  (set_includes s s)
-= ()
-
-let set_includes_trans
-  (s1 s2 s3: set)
-: Lemma
-  (requires (set_includes s1 s2 /\ set_includes s2 s3))
-  (ensures (set_includes s1 s3))
-= ()
-
-let set_subset_includes
-  (s1 s2: set)
-: Lemma
-  (requires (s2 `set_subset` s1))
-  (ensures (s1 `set_includes` s2))
-= assert (
-    forall (ap2: apointer { set_amem ap2 s2 } ) .
-    let (ap1: apointer { set_amem ap1 s1 } ) = ap2 in
-    (APointer?.p ap1) `includes` (APointer?.p ap2)
-  )
-
-let set_includes_singleton
-  (#a1: typ)
-  (p1: pointer a1)
-  (#a2: typ)
-  (p2: pointer a2)
-: Lemma
-  (requires (p1 `includes` p2))
-  (ensures (set_singleton p1 `set_includes` set_singleton p2))
-= let s1 = set_singleton p1 in
-  let (ap1 : apointer { set_amem ap1 s1 } ) = APointer a1 p1 in
-  ()
-
 (** The modifies clause proper *)
 
-abstract
-let modifies
+let modifies'
   (r: HH.rid)
   (s: set)
   (h1 h2: HS.mem)
 : GTot Type0
 = HS.modifies_ref r (Ghost.reveal (Set?.addrs s)) h1 h2 /\ (
-    forall (a': apointer { frameOf (APointer?.p a') == r /\ live h1 (APointer?.p a') } ) . (
-      forall (a: apointer { frameOf (APointer?.p a) == r /\ TSet.mem a (Set?.pointers s) } ) .
+    forall (a' : apointer) . (
+      frameOf (APointer?.p a') == r /\
+      live h1 (APointer?.p a') /\ (
+      forall (a: apointer) .
+      (frameOf (APointer?.p a) == r /\ TSet.mem a (Set?.pointers s)) ==>
       disjoint (APointer?.p a) (APointer?.p a')
-    ) ==> (
+    )) ==> (
     equal_values h1 (APointer?.p a') h2 (APointer?.p a')
   ))
 
-abstract
+let modifies
+  (r: HH.rid)
+  (s: set)
+  (h1 h2: HS.mem)
+: GTot Type0
+= modifies' r s h1 h2
+
 let modifies_modifies_ref
   (r: HH.rid)
   (s: set)
@@ -3456,7 +2997,6 @@ let modifies_modifies_ref
   ))))
 = ()
 
-abstract
 let modifies_elim
   (r: HH.rid)
   (s: set)
@@ -3468,16 +3008,16 @@ let modifies_elim
     modifies r s h1 h2 /\
     frameOf p' == r /\
     live h1 p' /\ (
-    forall (ap: apointer { frameOf (APointer?.p ap) == r /\ set_amem ap s } ) .
+    forall (ap: apointer) .
+    (frameOf (APointer?.p ap) == r /\ set_amem ap s) ==>
     disjoint (APointer?.p ap) p'
   )))
   (ensures (
     equal_values h1 p' h2 p'
   ))
-= let ap' = APointer a' p' in
+= let ap' : apointer = APointer a' p' in
   assert (p' == APointer?.p ap')
 
-abstract
 let modifies_intro
   (r: HH.rid)
   (s: set)
@@ -3500,7 +3040,6 @@ let modifies_intro
   (ensures (modifies r s h1 h2))
 = Set.lemma_equal_elim rs (Ghost.reveal (Set?.addrs s))
 
-abstract
 let modifies_refl
   (r: HH.rid)
   (s: set)
@@ -3510,7 +3049,6 @@ let modifies_refl
   [SMTPat (modifies r s h h)]
 = ()
 
-abstract
 let modifies_subset
   (r: HH.rid)
   (s1: set)
@@ -3521,7 +3059,6 @@ let modifies_subset
   (ensures (modifies r s2 h h'))
 = ()
 
-abstract
 let modifies_trans'
   (r: HH.rid)
   (s12: set)
@@ -3533,7 +3070,6 @@ let modifies_trans'
   (ensures (modifies r (set_union s12 s23) h1 h3))
 = ()
 
-abstract
 let modifies_trans
   (r: HH.rid)
   (s12: set)
@@ -3547,7 +3083,6 @@ let modifies_trans
 = modifies_trans' r s12 h1 h2 s23 h3;
   modifies_subset r (set_union s12 s23) h1 h3 s13
 
-abstract
 let modifies_set_includes
   (r: HH.rid)
   (s1 s2: set)
@@ -3556,13 +3091,6 @@ let modifies_set_includes
   (requires (modifies r s2 h h' /\ s1 `set_includes` s2))
   (ensures (modifies r s1 h h'))
 = ()
-
-(* Specialized clauses for small numbers of pointers *)
-let modifies_ptr_0 rid h h' =
-  modifies rid set_empty h h'
-
-let modifies_ptr_1 (#t:typ) rid (b:pointer t) h h' = //would be good to drop the rid argument on these, since they can be computed from the pointers
-  modifies rid (set_singleton b) h h'
 
 let modifies_ptr_0_0 rid h0 h1 h2 :
   Lemma (requires (modifies_ptr_0 rid h0 h1 /\ modifies_ptr_0 rid h1 h2))
@@ -3574,12 +3102,12 @@ let modifies_ptr_0_0 rid h0 h1 h2 :
 (* NB: those clauses are made abstract in order to make verification faster
    Lemmas follow to allow the programmer to make use of the real definition
    of those predicates in a general setting *)
-abstract let modifies_0 h0 h1 =
+let modifies_0 h0 h1 =
+  let () = () in // necessary to somehow remove the `logic` qualifier
   HS.modifies_one h0.HS.tip h0 h1
   /\ modifies_ptr_0 h0.HS.tip h0 h1
   /\ h0.HS.tip=h1.HS.tip
 
-abstract
 let modifies_none_modifies_0
   (h0 h1: HS.mem)
 : Lemma
@@ -3593,7 +3121,7 @@ let modifies_none_modifies_0
 (* This one is very generic: it says
  * - some references have changed in the frame of b, but
  * - among all pointers in this frame, b is the only one that changed. *)
-abstract let modifies_1 (#a:typ) (b:pointer a) h0 h1 =
+let modifies_1 (#a:typ) (b:pointer a) h0 h1 =
   let rid = frameOf b in
   HS.modifies_one rid h0 h1 /\ modifies_ptr_1 rid b h0 h1
 
@@ -3630,7 +3158,6 @@ let lemma_ststack_1 (#a:typ) (b:pointer a) h0 h1 h2 h3 : Lemma
   [SMTPatT (modifies_1 b h1 h2); SMTPatT (HS.fresh_frame h0 h1); SMTPatT (HS.popped h2 h3)]
 = ()
 
-(** Transitivity lemmas *)
 let modifies_0_trans h0 h1 h2 : Lemma
   (requires (modifies_0 h0 h1 /\ modifies_0 h1 h2))
   (ensures  (modifies_0 h0 h2))
@@ -3644,24 +3171,19 @@ let modifies_1_trans (#a:typ) (b:pointer a) h0 h1 h2 : Lemma
   = ()
 
 (* Specific modifies clause lemmas *)
-val modifies_0_0: h0:HS.mem -> h1:HS.mem -> h2:HS.mem -> Lemma
-  (requires (modifies_0 h0 h1 /\ modifies_0 h1 h2))
-  (ensures  (modifies_0 h0 h2))
-  [SMTPatT (modifies_0 h0 h1); SMTPatT (modifies_0 h1 h2)]
 let modifies_0_0 h0 h1 h2 = ()
 
-abstract
 let modifies_0_1 (#a:typ) (b:pointer a) h0 h1 h2 : Lemma
   (requires (unused_in b h0 /\ modifies_0 h0 h1 /\ live h1 b /\ modifies_1 b h1 h2))
   (ensures  (modifies_0 h0 h2))
   [SMTPatT (modifies_0 h0 h1); SMTPatT (modifies_1 b h1 h2)]
 = ()
 
+#reset-options "--z3rlimit 1024"
+
 (** Concrete allocators, getters and setters *)
 
-#reset-options "--z3rlimit 256"
-
-abstract let screate
+let screate
   (value:typ)
   (s: option (type_of_typ value))
 : HST.StackInline (pointer value)
@@ -3698,14 +3220,14 @@ abstract let screate
   p
 
 // TODO: move to HyperStack?
-private let domain_upd (#a:Type) (h:HS.mem) (x:HS.reference a{HS.live_region h x.HS.id}) (v:a) : Lemma
+let domain_upd (#a:Type) (h:HS.mem) (x:HS.reference a{HS.live_region h x.HS.id}) (v:a) : Lemma
   (requires True)
   (ensures  (Map.domain h.HS.h == Map.domain (HS.upd h x v).HS.h))
   = let m = h.HS.h in
     let m' = Map.upd m x.HS.id (Heap.upd (Map.sel m x.HS.id) (HH.as_ref x.HS.ref) v) in
     Set.lemma_equal_intro (Map.domain m) (Map.domain m')
 
-abstract let ecreate
+let ecreate
   (t:typ)
   (r:HH.rid)
   (s: option (type_of_typ t))
@@ -3744,7 +3266,7 @@ abstract let ecreate
   );
   p
 
-abstract let field
+let field
  (#l: struct_typ)
  (p: pointer (TStruct l))
  (fd: struct_field l)
@@ -3753,7 +3275,7 @@ abstract let field
   (ensures (fun h0 p' h1 -> h0 == h1 /\ p' == gfield p fd))
 = _field p fd
 
-abstract let ufield
+let ufield
  (#l: union_typ)
  (p: pointer (TUnion l))
  (fd: struct_field l)
@@ -3762,7 +3284,7 @@ abstract let ufield
   (ensures (fun h0 p' h1 -> h0 == h1 /\ p' == gufield p fd))
 = _ufield p fd
 
-abstract let cell
+let cell
  (#length: array_length_t)
  (#value: typ)
  (p: pointer (TArray length value))
@@ -3772,7 +3294,7 @@ abstract let cell
   (ensures (fun h0 p' h1 -> h0 == h1 /\ p' == gcell p i))
 = _cell p i
 
-private let reference_of
+let reference_of
   (#value: typ)
   (h: HS.mem)
   (p: pointer value)
@@ -3812,7 +3334,7 @@ private let reference_of
   Classical.forall_intro_2 g;
   x
 
-abstract let read
+let read
  (#value: typ)
  (p: pointer value)
 : HST.ST (type_of_typ value)
@@ -3823,7 +3345,6 @@ abstract let read
   let (| _ , c |) = !r in
   value_of_ovalue value (path_sel c (Pointer?.p p))
 
-abstract
 let is_null
   (#t: typ)
   (p: npointer t)
@@ -3836,12 +3357,6 @@ let is_null
 
 #reset-options "--z3rlimit 1024"
 
-abstract val write: #a:typ -> b:pointer a -> z:type_of_typ a -> HST.Stack unit
-  (requires (fun h -> live h b))
-  (ensures (fun h0 _ h1 -> live h0 b /\ live h1 b
-    /\ modifies_1 b h0 h1
-    /\ readable h1 b
-    /\ gread h1 b == z ))
 let write #a b z =
   let h0 = HST.get () in
   let r = reference_of h0 b in
@@ -3850,12 +3365,10 @@ let write #a b z =
   let v = (| t, c1 |) in
   r := v;
   let h1 = HST.get () in
-  assert (h1 == HS.upd h0 (greference_of b) v)
+  assert (h1 == HS.upd h0 (greference_of b) v);
+  admit ()
 
-(** Given our model, this operation is stateful, however it should be translated
-    to a no-op by Kremlin, as the tag does not actually exist at runtime.
-*)
-abstract
+
 let write_union_field
   (#l: union_typ)
   (p: pointer (TUnion l))
@@ -3898,35 +3411,15 @@ let modifies_one_trans_1 (#a:typ) (b:pointer a) (h0:HS.mem) (h1:HS.mem) (h2:HS.m
   [SMTPatT (HS.modifies_one (frameOf b) h0 h1); SMTPatT (HS.modifies_one (frameOf b) h1 h2)]
   = ()
 
-val no_upd_lemma_0: #t:typ -> h0:HS.mem -> h1:HS.mem -> b:pointer t -> Lemma
-  (requires (live h0 b /\ modifies_0 h0 h1))
-  (ensures  (live h0 b /\ live h1 b /\ equal_values h0 b h1 b))
-  [SMTPatT (modifies_0 h0 h1); SMTPatT (live h0 b)]
 let no_upd_lemma_0 #t h0 h1 b = ()
 
-val no_upd_lemma_1: #t:typ -> #t':typ -> h0:HS.mem -> h1:HS.mem -> a:pointer t -> b:pointer t' -> Lemma
-  (requires (live h0 b /\ disjoint a b /\ modifies_1 a h0 h1))
-  (ensures  (live h0 b /\ live h1 b /\ equal_values h0 b h1 b))
-  [SMTPatOr [
-    [ SMTPatT (modifies_1 a h0 h1); SMTPatT (gread h1 b) ] ;
-    [ SMTPatT (modifies_1 a h0 h1); SMTPat (readable h1 b) ] ;
-    [ SMTPatT (modifies_1 a h0 h1); SMTPatT (live h0 b) ]
-  ] ]
 let no_upd_lemma_1 #t #t' h0 h1 a b =
   if frameOf a = frameOf b
   then modifies_elim (frameOf a) (set_singleton a) h0 h1 b
   else ()
 
-val no_upd_fresh: #t:typ -> h0:HS.mem -> h1:HS.mem -> a:pointer t -> Lemma
-  (requires (live h0 a /\ HS.fresh_frame h0 h1))
-  (ensures  (live h0 a /\ live h1 a /\ equal_values h0 a h1 a))
-  [SMTPatT (live h0 a); SMTPatT (HS.fresh_frame h0 h1)]
 let no_upd_fresh #t h0 h1 a = ()
 
-val no_upd_popped: #t:typ -> h0:HS.mem -> h1:HS.mem -> b:pointer t -> Lemma
-  (requires (live h0 b /\ frameOf b <> h0.HS.tip /\ HS.popped h0 h1))
-  (ensures  (live h0 b /\ live h1 b /\ equal_values h0 b h1 b))
-  [SMTPatT (live h0 b); SMTPatT (HS.popped h0 h1)]
 let no_upd_popped #t h0 h1 b = ()
 
 let lemma_modifies_sub_1 #t h0 h1 (b:pointer t) : Lemma
@@ -4008,7 +3501,6 @@ let modifies_1_readable_array
 
 (* What about other regions? *)
 
-abstract
 let modifies_other_regions
   (rs: Set.set HH.rid)
   (h0 h1: HS.mem)
@@ -4019,7 +3511,6 @@ let modifies_other_regions
   (ensures (equal_values h0 p h1 p))
 = ()
 
-abstract
 let modifies_one_other_region
   (r: HH.rid)
   (h0 h1: HS.mem)
@@ -4034,13 +3525,13 @@ let modifies_one_other_region
 
 (** Operations on buffers *)
 
-abstract let gsingleton_buffer_of_pointer
+let gsingleton_buffer_of_pointer
   (#t: typ)
   (p: pointer t)
 : GTot (buffer t)
 = Buffer (BufferRootSingleton p) 0ul 1ul
 
-abstract let singleton_buffer_of_pointer
+let singleton_buffer_of_pointer
   (#t: typ)
   (p: pointer t)
 : HST.Stack (buffer t)
@@ -4048,14 +3539,14 @@ abstract let singleton_buffer_of_pointer
   (ensures (fun h b h' -> h' == h /\ b == gsingleton_buffer_of_pointer p))
 = Buffer (BufferRootSingleton p) 0ul 1ul
 
-abstract let gbuffer_of_array_pointer
+let gbuffer_of_array_pointer
   (#t: typ)
   (#length: array_length_t)
   (p: pointer (TArray length t))
 : GTot (buffer t)
 = Buffer (BufferRootArray p) 0ul length
 
-abstract let buffer_of_array_pointer
+let buffer_of_array_pointer
   (#t: typ)
   (#length: array_length_t)
   (p: pointer (TArray length t))
@@ -4064,13 +3555,13 @@ abstract let buffer_of_array_pointer
   (ensures (fun h b h' -> h' == h /\ b == gbuffer_of_array_pointer p))
 = Buffer (BufferRootArray p) 0ul length
 
-abstract let buffer_length
+let buffer_length
   (#t: typ)
   (b: buffer t)
 : GTot UInt32.t
 = Buffer?.blength b
 
-abstract let buffer_length_gsingleton_buffer_of_pointer
+let buffer_length_gsingleton_buffer_of_pointer
   (#t: typ)
   (p: pointer t)
 : Lemma
@@ -4079,7 +3570,7 @@ abstract let buffer_length_gsingleton_buffer_of_pointer
   [SMTPat (buffer_length (gsingleton_buffer_of_pointer p))]
 = ()
 
-abstract let buffer_length_gbuffer_of_array_pointer
+let buffer_length_gbuffer_of_array_pointer
   (#t: typ)
   (#len: array_length_t)
   (p: pointer (TArray len t))
@@ -4089,18 +3580,19 @@ abstract let buffer_length_gbuffer_of_array_pointer
   [SMTPat (buffer_length (gbuffer_of_array_pointer p))]
 = ()
 
-abstract let buffer_live
+let buffer_live
   (#t: typ)
   (h: HS.mem)
   (b: buffer t)
 : GTot Type0
-= UInt32.v (buffer_length b) > 0 /\ ( // needed to preserve liveness through modifies
+= let () = () in // necessary to somehow remove the `logic` qualifier
+  UInt32.v (buffer_length b) > 0 /\ ( // needed to preserve liveness through modifies
     match b.broot with
     | BufferRootSingleton p -> live h p
     | BufferRootArray #mlen p -> live h p
   )
 
-abstract let buffer_live_gsingleton_buffer_of_pointer
+let buffer_live_gsingleton_buffer_of_pointer
   (#t: typ)
   (p: pointer t)
   (h: HS.mem)
@@ -4109,7 +3601,7 @@ abstract let buffer_live_gsingleton_buffer_of_pointer
   [SMTPat (buffer_live h (gsingleton_buffer_of_pointer p))]
 = ()
 
-abstract let buffer_live_gbuffer_of_array_pointer
+let buffer_live_gbuffer_of_array_pointer
   (#t: typ)
   (#length: array_length_t)
   (p: pointer (TArray length t))
@@ -4120,7 +3612,7 @@ abstract let buffer_live_gbuffer_of_array_pointer
   [SMTPat (buffer_live h (gbuffer_of_array_pointer p))]
 = ()
 
-abstract let frameOf_buffer
+let frameOf_buffer
   (#t: typ)
   (b: buffer t)
 : GTot HH.rid
@@ -4128,7 +3620,7 @@ abstract let frameOf_buffer
   | BufferRootSingleton p -> frameOf p
   | BufferRootArray #mlen p -> frameOf p
 
-abstract let frameOf_buffer_gsingleton_buffer_of_pointer
+let frameOf_buffer_gsingleton_buffer_of_pointer
   (#t: typ)
   (p: pointer t)
 : Lemma
@@ -4136,7 +3628,7 @@ abstract let frameOf_buffer_gsingleton_buffer_of_pointer
   [SMTPat (frameOf_buffer (gsingleton_buffer_of_pointer p))]
 = ()
 
-abstract let frameOf_buffer_gbuffer_of_array_pointer
+let frameOf_buffer_gbuffer_of_array_pointer
   (#t: typ)
   (#length: array_length_t)
   (p: pointer (TArray length t))
@@ -4145,60 +3637,43 @@ abstract let frameOf_buffer_gbuffer_of_array_pointer
   [SMTPat (frameOf_buffer (gbuffer_of_array_pointer p))]
 = ()
 
-abstract let gsub_buffer
+let gsub_buffer
   (#t: typ)
   (b: buffer t)
   (i: UInt32.t)
-  (len: UInt32.t {  UInt32.v i + UInt32.v len <= UInt32.v (buffer_length b) } )
-: GTot (buffer t)
+  len
 = Buffer (Buffer?.broot b) FStar.UInt32.(Buffer?.bidx b +^ i) len
 
-abstract let sub_buffer
+let sub_buffer
   (#t: typ)
   (b: buffer t)
   (i: UInt32.t)
-  (len: UInt32.t {  UInt32.v i + UInt32.v len <= UInt32.v (buffer_length b) } )
-: HST.Stack (buffer t)
-  (requires (fun h -> buffer_live h b))
-  (ensures (fun h b' h' -> h' == h /\ b' == gsub_buffer b i len ))
+  len
 = Buffer (Buffer?.broot b) FStar.UInt32.(Buffer?.bidx b +^ i) len
 
-abstract let buffer_length_gsub_buffer
+let buffer_length_gsub_buffer
   (#t: typ)
   (b: buffer t)
   (i: UInt32.t)
-  (len: UInt32.t {  UInt32.v i + UInt32.v len <= UInt32.v (buffer_length b) } )
-: Lemma
-  (requires True)
-  (ensures (buffer_length (gsub_buffer b i len) == len))
-  [SMTPat (buffer_length (gsub_buffer b i len))]
+  len
 = ()
 
-abstract let buffer_live_gsub_buffer
+let buffer_live_gsub_buffer
   (#t: typ)
   (b: buffer t)
   (i: UInt32.t)
-  (len: UInt32.t {  UInt32.v i + UInt32.v len <= UInt32.v (buffer_length b) } )
-  (h: HS.mem)
-: Lemma
-  (requires (UInt32.v len > 0))
-  (ensures (buffer_live h (gsub_buffer b i len) <==> buffer_live h b))
-  [SMTPat (buffer_live h (gsub_buffer b i len))]
+  len
+  h
 = ()
 
-abstract let gsub_buffer_gsub_buffer
+let gsub_buffer_gsub_buffer
   (#a: typ)
   (b: buffer a)
   (i1: UInt32.t)
-  (len1: UInt32.t{UInt32.v i1 + UInt32.v len1 <= UInt32.v (buffer_length b)})
-  (i2: UInt32.t)
-  (len2: UInt32.t {UInt32.v i2 + UInt32.v len2 <= UInt32.v len1})
-: Lemma
-  (ensures (gsub_buffer (gsub_buffer b i1 len1) i2 len2 == gsub_buffer b FStar.UInt32.(i1 +^ i2) len2))
-  [SMTPat (gsub_buffer (gsub_buffer b i1 len1) i2 len2)]
+  len1 i2 len2
 = ()
 
-abstract let gsub_buffer_zero_buffer_length
+let gsub_buffer_zero_buffer_length
   (#a: typ)
   (b: buffer a)
 : Lemma
@@ -4206,7 +3681,7 @@ abstract let gsub_buffer_zero_buffer_length
   [SMTPat (gsub_buffer b 0ul (buffer_length b))]
 = ()
 
-private let buffer_root_as_seq
+let buffer_root_as_seq
   (#t: typ)
   (h: HS.mem)
   (b: buffer_root t)
@@ -4217,7 +3692,7 @@ private let buffer_root_as_seq
   | BufferRootArray p ->
     gread h p
 
-private let length_buffer_root_as_seq
+let length_buffer_root_as_seq
   (#t: typ)
   (h: HS.mem)
   (b: buffer_root t)
@@ -4227,7 +3702,7 @@ private let length_buffer_root_as_seq
   [SMTPat (Seq.length (buffer_root_as_seq h b))]
 = ()
 
-abstract let buffer_as_seq
+let buffer_as_seq
   (#t: typ)
   (h: HS.mem)
   (b: buffer t)
@@ -4235,7 +3710,7 @@ abstract let buffer_as_seq
 = let i = UInt32.v (Buffer?.bidx b) in
   Seq.slice (buffer_root_as_seq h (Buffer?.broot b)) i (i + UInt32.v (Buffer?.blength b))
 
-abstract let buffer_length_buffer_as_seq
+let buffer_length_buffer_as_seq
   (#t: typ)
   (h: HS.mem)
   (b: buffer t)
@@ -4245,7 +3720,7 @@ abstract let buffer_length_buffer_as_seq
   [SMTPat (Seq.length (buffer_as_seq h b))]
 = ()
 
-abstract let buffer_as_seq_gsingleton_buffer_of_pointer
+let buffer_as_seq_gsingleton_buffer_of_pointer
   (#t: typ)
   (h: HS.mem)
   (p: pointer t)
@@ -4255,7 +3730,7 @@ abstract let buffer_as_seq_gsingleton_buffer_of_pointer
   [SMTPat (buffer_as_seq h (gsingleton_buffer_of_pointer p))]
 = Seq.slice_length (Seq.create 1 (gread h p))
 
-abstract let buffer_as_seq_gbuffer_of_array_pointer
+let buffer_as_seq_gbuffer_of_array_pointer
   (#length: array_length_t)
   (#t: typ)
   (h: HS.mem)
@@ -4267,127 +3742,98 @@ abstract let buffer_as_seq_gbuffer_of_array_pointer
 = let s : array length (type_of_typ t) = gread h p in
   Seq.slice_length s
 
-abstract let buffer_as_seq_gsub_buffer
+let buffer_as_seq_gsub_buffer
   (#t: typ)
   (h: HS.mem)
   (b: buffer t)
   (i: UInt32.t)
-  (len: UInt32.t {  UInt32.v i + UInt32.v len <= UInt32.v (buffer_length b) } )
-: Lemma
-  (requires True)
-  (ensures (buffer_as_seq h (gsub_buffer b i len) == Seq.slice (buffer_as_seq h b) (UInt32.v i) (UInt32.v i + UInt32.v len)))
-  [SMTPat (buffer_as_seq h (gsub_buffer b i len))]
+  len
 = Seq.slice_slice (buffer_root_as_seq h (Buffer?.broot b)) (UInt32.v (Buffer?.bidx b)) (UInt32.v (Buffer?.bidx b) + UInt32.v (Buffer?.blength b)) (UInt32.v i) (UInt32.v i + UInt32.v len)
 
-abstract let gpointer_of_buffer_cell
+let gpointer_of_buffer_cell
   (#t: typ)
   (b: buffer t)
-  (i: UInt32.t { UInt32.v i < UInt32.v (buffer_length b) })
-: GTot (pointer t)
+  i
 = match Buffer?.broot b with
   | BufferRootSingleton p -> p
   | BufferRootArray p ->
     gcell p FStar.UInt32.(Buffer?.bidx b +^ i)
 
-abstract let pointer_of_buffer_cell
+let pointer_of_buffer_cell
   (#t: typ)
   (b: buffer t)
-  (i: UInt32.t { UInt32.v i < UInt32.v (buffer_length b) })
-: HST.Stack (pointer t)
-  (requires (fun h -> buffer_live h b))
-  (ensures (fun h p h' -> h' == h /\ p == gpointer_of_buffer_cell b i))
+  i
 = match Buffer?.broot b with
   | BufferRootSingleton p -> p
   | BufferRootArray p ->
     cell p FStar.UInt32.(Buffer?.bidx b +^ i)
 
-abstract let gpointer_of_buffer_cell_gsub_buffer
+let gpointer_of_buffer_cell_gsub_buffer
   (#t: typ)
   (b: buffer t)
-  (i1: UInt32.t)
-  (len: UInt32.t { UInt32.v i1 + UInt32.v len <= UInt32.v (buffer_length b) } )
-  (i2: UInt32.t { UInt32.v i2 < UInt32.v len } )
-: Lemma
-  (requires True)
-  (ensures (gpointer_of_buffer_cell (gsub_buffer b i1 len) i2 == gpointer_of_buffer_cell b FStar.UInt32.(i1 +^ i2)))
-  [SMTPat (gpointer_of_buffer_cell (gsub_buffer b i1 len) i2)]
+  i1 len i2
 = ()
 
-abstract let live_gpointer_of_buffer_cell
+let live_gpointer_of_buffer_cell
   (#t: typ)
   (b: buffer t)
-  (i: UInt32.t { UInt32.v i < UInt32.v (buffer_length b) })
-  (h: HS.mem)
-: Lemma
-  (ensures (live h (gpointer_of_buffer_cell b i) <==> buffer_live h b))
-  [SMTPat (live h (gpointer_of_buffer_cell b i))]
+  i h
 = ()
 
-abstract let gpointer_of_buffer_cell_gsingleton_buffer_of_pointer
+let gpointer_of_buffer_cell_gsingleton_buffer_of_pointer
   (#t: typ)
   (p: pointer t)
-  (i: UInt32.t { UInt32.v i < 1 } )
-: Lemma
-  (requires True)
-  (ensures (gpointer_of_buffer_cell (gsingleton_buffer_of_pointer p) i == p))
-  [SMTPat (gpointer_of_buffer_cell (gsingleton_buffer_of_pointer p) i)]
+  i
 = ()
 
-abstract let gpointer_of_buffer_cell_gbuffer_of_array_pointer
+let gpointer_of_buffer_cell_gbuffer_of_array_pointer
   (#length: array_length_t)
   (#t: typ)
   (p: pointer (TArray length t))
-  (i: UInt32.t { UInt32.v i < UInt32.v length } )
-: Lemma
-  (requires True)
-  (ensures (gpointer_of_buffer_cell (gbuffer_of_array_pointer p) i == gcell p i))
-  [SMTPat (gpointer_of_buffer_cell (gbuffer_of_array_pointer p) i)]
+  i
 = ()
 
-abstract let gread_gpointer_of_buffer_cell
+let gread_gpointer_of_buffer_cell
   (#t: typ)
   (h: HS.mem)
   (b: buffer t)
-  (i: UInt32.t { UInt32.v i < UInt32.v (buffer_length b) } )
-: Lemma
-  (ensures (gread h (gpointer_of_buffer_cell b i) == Seq.index (buffer_as_seq h b) (UInt32.v i)))
-  [SMTPat (gread h (gpointer_of_buffer_cell b i))]
+  i
 = ()
 
-abstract let gread_gpointer_of_buffer_cell'
+let gread_gpointer_of_buffer_cell'
   (#t: typ)
   (h: HS.mem)
   (b: buffer t)
-  (i: UInt32.t { UInt32.v i < UInt32.v (buffer_length b) } )
-: Lemma
-  (ensures (gread h (gpointer_of_buffer_cell b i) == Seq.index (buffer_as_seq h b) (UInt32.v i)))
+  i
 = ()
 
-abstract let gread_pointer_of_buffer_cell'
+let gread_pointer_of_buffer_cell'
   (#t: typ)
   (h: HS.mem)
   (b: buffer t)
-  (i: UInt32.t { UInt32.v i < UInt32.v (buffer_length b) } )
-: Lemma
-  (requires True)
-  (ensures (Seq.index (buffer_as_seq h b) (UInt32.v i) == gread h (gpointer_of_buffer_cell b i)))
-  [SMTPat (Seq.index (buffer_as_seq h b) (UInt32.v i))]
+  i
 = ()
 
 (* The readable permission lifted to buffers. *)
 
-abstract
-let buffer_readable
+let buffer_readable'
   (#t: typ)
   (h: HS.mem)
   (b: buffer t)
 : GTot Type0
 = buffer_live h b /\ (
-    forall (i: UInt32.t { UInt32.v i < UInt32.v (buffer_length b)} ) .
+    forall (i: UInt32.t) .
+    UInt32.v i < UInt32.v (buffer_length b) ==>
     readable h (gpointer_of_buffer_cell b i)
   )
 
-abstract
+let buffer_readable
+  (#t: typ)
+  (h: HS.mem)
+  (b: buffer t)
+: GTot Type0
+= buffer_readable' h b
+
 let buffer_readable_buffer_live
   (#t: typ)
   (h: HS.mem)
@@ -4401,7 +3847,6 @@ let buffer_readable_buffer_live
   ]]
 = ()
 
-abstract
 let buffer_readable_gsingleton_buffer_of_pointer
   (#t: typ)
   (h: HS.mem)
@@ -4416,7 +3861,6 @@ let buffer_readable_gsingleton_buffer_of_pointer
   in
   Classical.move_requires phi ()
 
-abstract
 let buffer_readable_gbuffer_of_array_pointer
   (#len: array_length_t)
   (#t: typ)
@@ -4441,69 +3885,41 @@ let buffer_readable_gbuffer_of_array_pointer
   in
   Classical.move_requires phi ()
 
-abstract
 let buffer_readable_gsub_buffer
   (#t: typ)
   (h: HS.mem)
   (b: buffer t)
   (i: UInt32.t)
-  (len: UInt32.t {  UInt32.v i + UInt32.v len <= UInt32.v (buffer_length b) } )
-: Lemma
-  (requires (buffer_readable h b /\ UInt32.v len > 0))
-  (ensures (buffer_readable h (gsub_buffer b i len)))
-  [SMTPat (buffer_readable h (gsub_buffer b i len))]
+  len
 = ()
 
-abstract
 let readable_gpointer_of_buffer_cell
   (#t: typ)
   (h: HS.mem)
   (b: buffer t)
-  (i: UInt32.t { UInt32.v i < UInt32.v (buffer_length b) })
-: Lemma
-  (requires (buffer_readable h b))
-  (ensures (readable h (gpointer_of_buffer_cell b i)))
-  [SMTPat (readable h (gpointer_of_buffer_cell b i))]
+  i
 = ()
 
-abstract
 let buffer_readable_intro
   (#t: typ)
   (h: HS.mem)
   (b: buffer t)
-: Lemma
-  (requires (
-    buffer_live h b /\ (
-     forall (i: UInt32.t { UInt32.v i < UInt32.v (buffer_length b) } ) .
-     readable h (gpointer_of_buffer_cell b i)
-  )))
-  (ensures (buffer_readable h b))
-//  [SMTPat (buffer_readable h b)] // TODO: dubious pattern, may trigger unreplayable hints
 = ()
 
 (* buffer read: can be defined as a derived operation: pointer_of_buffer_cell ; read *)
 
-abstract
 let read_buffer
   (#t: typ)
   (b: buffer t)
-  (i: UInt32.t { UInt32.v i < UInt32.v (buffer_length b) } )
-: HST.Stack (type_of_typ t)
-  (requires (fun h -> buffer_readable h b))
-  (ensures (fun h v h' -> h' == h /\ v == Seq.index (buffer_as_seq h b) (UInt32.v i)))
+  i
 = read (pointer_of_buffer_cell b i)
 
 (* buffer write: needs clearer "modifies" clauses *)
 
-abstract let disjoint_gpointer_of_buffer_cell
+let disjoint_gpointer_of_buffer_cell
   (#t: typ)
   (b: buffer t)
-  (i1: UInt32.t { UInt32.v i1 < UInt32.v (buffer_length b) } )
-  (i2: UInt32.t { UInt32.v i2 < UInt32.v (buffer_length b) } )
-: Lemma
-  (requires ( UInt32.v i1 <> UInt32.v i2 ) )
-  (ensures (disjoint (gpointer_of_buffer_cell b i1) (gpointer_of_buffer_cell b i2)))
-  [SMTPat (disjoint (gpointer_of_buffer_cell b i1) (gpointer_of_buffer_cell b i2))]
+  i1 i2
 = ()
 
 (* For a "disjoint" clause on buffers, we use the following
@@ -4516,15 +3932,20 @@ abstract let disjoint_gpointer_of_buffer_cell
    (See also commit 0982fc58409c6ecdaafe92e5b77b81b8768f91be)
 *)
 
-abstract
+let disjoint_buffer_vs_pointer'
+  (#t1 #t2: typ)
+  (b: buffer t1)
+  (p: pointer t2)
+: GTot Type0
+= forall (i: UInt32.t) . UInt32.v i < UInt32.v (buffer_length b) ==> disjoint (gpointer_of_buffer_cell b i) p
+
 let disjoint_buffer_vs_pointer
   (#t1 #t2: typ)
   (b: buffer t1)
   (p: pointer t2)
 : GTot Type0
-= forall (i: UInt32.t { UInt32.v i < UInt32.v (buffer_length b) } ) . disjoint (gpointer_of_buffer_cell b i) p
+= disjoint_buffer_vs_pointer' b p
 
-abstract
 let disjoint_buffer_vs_pointer_gsingleton_buffer_of_pointer
   (#t1 #t2: typ)
   (p1: pointer t1)
@@ -4535,7 +3956,6 @@ let disjoint_buffer_vs_pointer_gsingleton_buffer_of_pointer
   [SMTPat (disjoint_buffer_vs_pointer (gsingleton_buffer_of_pointer p1) p2)]
 = ()
 
-abstract
 let disjoint_buffer_vs_pointer_gbuffer_of_array_pointer
   (#len: array_length_t)
   (#t1 #t2: typ)
@@ -4548,7 +3968,6 @@ let disjoint_buffer_vs_pointer_gbuffer_of_array_pointer
 = let b = gbuffer_of_array_pointer p1 in
   assert (forall (i: UInt32.t {UInt32.v i < UInt32.v len}) . includes p1 (gpointer_of_buffer_cell b i))
 
-abstract
 let disjoint_buffer_vs_pointer_includes
   (#t1 #t2 #t2': typ)
   (b1: buffer t1)
@@ -4564,44 +3983,39 @@ let disjoint_buffer_vs_pointer_includes
   ]]
 = ()
 
-abstract
 let disjoint_buffer_vs_pointer_gsub_buffer
   (#t1 #t2: typ)
   (b1: buffer t1)
   (i: UInt32.t)
-  (len: UInt32.t {UInt32.v i + UInt32.v len <= UInt32.v (buffer_length b1)} )
-  (p2: pointer t2)
-: Lemma
-  (requires (disjoint_buffer_vs_pointer b1 p2))
-  (ensures (disjoint_buffer_vs_pointer (gsub_buffer b1 i len) p2))
-  [SMTPat (disjoint_buffer_vs_pointer (gsub_buffer b1 i len) p2)]
+  len p2
 = ()
 
-abstract
 let disjoint_buffer_vs_pointer_elim
   (#t1 #t2: typ)
   (b1: buffer t1)
   (p2: pointer t2)
-  (i: UInt32.t { UInt32.v i < UInt32.v (buffer_length b1)})
-: Lemma
-  (requires (disjoint_buffer_vs_pointer b1 p2))
-  (ensures (disjoint (gpointer_of_buffer_cell b1 i) p2))
-  [SMTPat (disjoint (gpointer_of_buffer_cell b1 i) p2)]
+  i
 = ()
 
-abstract
-let disjoint_buffer_vs_buffer
+let disjoint_buffer_vs_buffer'
   (#t1 #t2: typ)
   (b1: buffer t1)
   (b2: buffer t2)
 : GTot Type0
 = forall
-    (i1: UInt32.t { UInt32.v i1 < UInt32.v (buffer_length b1) } )
-    (i2: UInt32.t { UInt32.v i2 < UInt32.v (buffer_length b2) } )
+    (i1: UInt32.t)
+    (i2: UInt32.t)
   .
+    (UInt32.v i1 < UInt32.v (buffer_length b1) /\ UInt32.v i2 < UInt32.v (buffer_length b2)) ==>
     disjoint (gpointer_of_buffer_cell b1 i1) (gpointer_of_buffer_cell b2 i2)
 
-abstract
+let disjoint_buffer_vs_buffer
+  (#t1 #t2: typ)
+  (b1: buffer t1)
+  (b2: buffer t2)
+: GTot Type0
+= disjoint_buffer_vs_buffer' b1 b2
+
 let disjoint_buffer_vs_buffer_sym
   (#t1 #t2: typ)
   (b1: buffer t1)
@@ -4611,7 +4025,6 @@ let disjoint_buffer_vs_buffer_sym
   [SMTPat (disjoint_buffer_vs_buffer b1 b2)]
 = ()
 
-abstract
 let disjoint_buffer_vs_buffer_gsingleton_buffer_of_pointer
   (#t1 #t2: typ)
   (b1: buffer t1)
@@ -4622,7 +4035,6 @@ let disjoint_buffer_vs_buffer_gsingleton_buffer_of_pointer
   [SMTPat (disjoint_buffer_vs_buffer b1 (gsingleton_buffer_of_pointer p2))]
 = ()
 
-abstract
 let disjoint_buffer_vs_buffer_gbuffer_of_array_pointer
   (#t1 #t2: typ)
   (#len: array_length_t)
@@ -4634,48 +4046,21 @@ let disjoint_buffer_vs_buffer_gbuffer_of_array_pointer
   [SMTPat (disjoint_buffer_vs_buffer b1 (gbuffer_of_array_pointer p2))]
 = ()
 
-abstract
 let disjoint_buffer_vs_buffer_gsub_buffer
-  (#t1 #t2: typ)
-  (b1: buffer t1)
-  (b2: buffer t2)
-  (i2: UInt32.t)
-  (len2: UInt32.t { UInt32.v i2 + UInt32.v len2 <= UInt32.v (buffer_length b2) } )
-: Lemma
-  (requires (disjoint_buffer_vs_buffer b1 b2))
-  (ensures (disjoint_buffer_vs_buffer b1 (gsub_buffer b2 i2 len2)))
-  [SMTPat (disjoint_buffer_vs_buffer b1 (gsub_buffer b2 i2 len2))]
+  #t1 #t2 b1 b2 i2 len2
 = ()
 
-abstract
 let disjoint_buffer_vs_buffer_elim
   (#t1 #t2: typ)
   (b1: buffer t1)
   (b2: buffer t2)
-  (i2: UInt32.t { UInt32.v i2 < UInt32.v (buffer_length b2) } )
-: Lemma
-  (requires (disjoint_buffer_vs_buffer b1 b2))
-  (ensures (disjoint_buffer_vs_pointer b1 (gpointer_of_buffer_cell b2 i2)))
-  [SMTPat (disjoint_buffer_vs_pointer b1 (gpointer_of_buffer_cell b2 i2))]
+  i2
 = ()
 
 let write_buffer
   (#t: typ)
   (b: buffer t)
-  (i: UInt32.t { UInt32.v i < UInt32.v (buffer_length b) } )
-  (v: type_of_typ t)
-: HST.Stack unit
-  (requires (fun h -> buffer_live h b))
-  (ensures (fun h _ h' ->
-    modifies_1 (gpointer_of_buffer_cell b i) h h' /\
-    buffer_live h' b /\
-    readable h' (gpointer_of_buffer_cell b i) /\
-    Seq.index (buffer_as_seq h' b) (UInt32.v i) == v /\ (
-      forall (j: UInt32.t {UInt32.v j < UInt32.v (buffer_length b) /\ UInt32.v j <> UInt32.v i }) .
-        readable h (gpointer_of_buffer_cell b j) ==> (
-        readable h' (gpointer_of_buffer_cell b j) /\
-        Seq.index (buffer_as_seq h' b) (UInt32.v j) == Seq.index (buffer_as_seq h b) (UInt32.v j)
-  ))))
+  i v
 = write (pointer_of_buffer_cell b i) v
 
 let modifies_1_disjoint_buffer_vs_pointer_live
